theories/LogicalRelation/Definition/Ne.v
@@ -37,13 +37,23 @@ End neRedTy.
 Export neRedTy(neRedTy, Build_neRedTy).
 Notation "[ Γ ||-ne A ≅ B ]" := (neRedTy Γ A B).
 
+#[program]
+Instance neRedTyWhRedTy `{GenericTypingProperties} {Γ} : WhRedTyRel Γ (neRedTy Γ) :=
+  {| whredtyL := fun A B RAB => neRedTy.whredL RAB ;
+     whredtyR := fun A B RAB => neRedTy.whredR RAB ;
+  |}.
+Next Obligation.
+  destruct h.
+  eapply convty_term, convtm_convneu; tea; constructor.
+Qed.
+
 
 Module neRedTmEq.
 
   Record neRedTmEq `{ta : tag}
     `{WfType ta} `{RedType ta}
     `{Typing ta} `{ConvType ta} `{ConvTerm ta} `{ConvNeuConv ta} `{RedTerm ta}
-    {Γ : context} {t u A B : term} {R : [ Γ ||-ne A ≅ B]}
+    {Γ : context} {A B : term} {R : [ Γ ||-ne A ≅ B]} {t u  : term}
   : Set := {
     termL     : term;
     termR     : term;
@@ -52,27 +62,36 @@ Module neRedTmEq.
     eq : [ Γ |- termL ~ termR : R.(neRedTy.tyL)] ;
   }.
 
-  Arguments neRedTmEq {_ _ _ _ _ _ _ _ _} _ _ {_ _} _.
+  Arguments neRedTmEq {_ _ _ _ _ _ _ _ _ _ _} _ _ _.
 
   Definition whredL `{GenericTypingProperties} {Γ : context} {t u A B : term} {R : [ Γ ||-ne A ≅ B]} :
-    neRedTmEq t u R -> [Γ |- t ↘  R.(neRedTy.tyL)].
+    neRedTmEq R t u -> [Γ |- t ↘  R.(neRedTy.tyL)].
   Proof.  intros []; econstructor; tea; constructor; now eapply convneu_whne. Defined.
 
   Definition whredR `{GenericTypingProperties} {Γ : context} {t u A B : term} {R : [ Γ ||-ne A ≅ B]} :
-    neRedTmEq t u R -> [Γ |- u ↘  R.(neRedTy.tyL)].
+    neRedTmEq R t u -> [Γ |- u ↘  R.(neRedTy.tyL)].
   Proof. intros []; econstructor; tea; constructor; eapply convneu_whne; now symmetry. Defined.
 
 End neRedTmEq.
 
 Export neRedTmEq(neRedTmEq, Build_neRedTmEq).
-Notation "[ Γ ||-ne t ≅ u : A | R ] " := (neRedTmEq (Γ:=Γ) (A:=A) t u R).
+Notation "[ Γ ||-ne t ≅ u : A | R ] " := (neRedTmEq (Γ:=Γ) (A:=A) R t u).
 
+#[program]
+Instance neRedTmWhRedTm `{GenericTypingProperties} {Γ A B} (R : [Γ ||-ne A ≅ B]) : WhRedTmRel Γ (neRedTy.tyL R) (neRedTmEq R) :=
+  {| whredtmL := fun t u Rtu => neRedTmEq.whredL Rtu ;
+     whredtmR := fun t u Rtu => neRedTmEq.whredR Rtu ;
+  |}.
+Next Obligation.
+  destruct h; cbn; eapply convtm_convneu; tea.
+  destruct R; cbn in *; constructor; now eapply convneu_whne.
+Qed.
 
 (** ** Reducibility of neutrals at an arbitrary type *)
 
 Module NeNf.
 
-  Record RedTmEq `{ta : tag} `{Typing ta} `{ConvNeuConv ta} {Γ k l A} : Set :=
+  Record RedTmEq `{ta : tag} `{Typing ta} `{ConvNeuConv ta} {Γ A k l} : Set :=
     {
       tyL : [Γ |- k : A] ;
       tyR : [Γ |- l : A] ;
@@ -82,7 +101,7 @@ Module NeNf.
   Arguments RedTmEq {_ _ _}.
 
   Definition whredL `{GenericTypingProperties} {Γ : context} {t u A : term} :
-    RedTmEq Γ t u A -> [Γ |- t ↘  A].
+    RedTmEq Γ A t u -> [Γ |- t ↘  A].
   Proof.
     intros []; econstructor.
     1: now eapply redtmwf_refl.
@@ -90,7 +109,7 @@ Module NeNf.
   Defined.
 
   Definition whredR `{GenericTypingProperties} {Γ : context} {t u A : term} :
-    RedTmEq Γ t u A -> [Γ |- u ↘  A].
+    RedTmEq Γ A t u -> [Γ |- u ↘  A].
   Proof.
     intros []; econstructor.
     1: now eapply redtmwf_refl.
@@ -98,7 +117,7 @@ Module NeNf.
   Defined.
 
   Definition conv_ `{GenericTypingProperties} {Γ : context} {t u A B : term} :
-    [Γ |- A ≅ B] -> RedTmEq Γ t u A -> RedTmEq Γ t u B.
+    [Γ |- A ≅ B] -> RedTmEq Γ A t u -> RedTmEq Γ B t u.
   Proof.
     intros ? []; econstructor.
     1,2: now eapply ty_conv.
@@ -107,5 +126,14 @@ Module NeNf.
 
 End NeNf.
 
-Notation "[ Γ ||-NeNf k ≅ l : A ]" := (NeNf.RedTmEq Γ k l A) (at level 0, Γ, k, l, A at level 50).
+Notation "[ Γ ||-NeNf k ≅ l : A ]" := (NeNf.RedTmEq Γ A k l) (at level 0, Γ, k, l, A at level 50).
 
+
+#[program]
+Instance NeNfWhRedTm `{GenericTypingProperties} {Γ A} (posA : isPosType A) : WhRedTmRel Γ A (NeNf.RedTmEq Γ A) :=
+  {| whredtmL := fun t u Rtu => NeNf.whredL Rtu ;
+     whredtmR := fun t u Rtu => NeNf.whredR Rtu ;
+  |}.
+Next Obligation.
+  destruct h; now eapply convtm_convneu.
+Defined.
