theories/LogicalRelation/Irrelevance.v
@@ -2,39 +2,63 @@
 From Coq Require Import CRelationClasses.
 From LogRel Require Import Utils Syntax.All GenericTyping LogicalRelation.
 From LogRel.LogicalRelation Require Import Induction Escape.
- (* ShapeView Reflexivity . *)
 
 Set Universe Polymorphism.
 Set Printing Universes.
 Set Printing Primitive Projection Parameters.
 
+(** We show a general version of irrelevance, saying that the relation associated to
+  two witnesses of reducibility of A (Γ ||-<l1> A ≅ B1 and Γ ||-<l2> A ≅ B2) coincide. *)
+(** Interestingly, we also show irrelevance with respect to universe levels, which is crucial
+in later parts of the development, where this avoids creating spurious constraints on universe levels.*)
+
+Axiom todo@{u}: forall {A:Type@{u}}, A.
 
 Section Irrelevance.
   Context `{GenericTypingProperties}.
 
   Universe v.
-
   Notation "A <≈> B" := (prod@{v v} (A -> B) (B -> A)) (at level 90).
 
+  Section Defs.
+  Universe i j k l i' j' k' l'.
 
-  Let irr {Γ l1 l2 A B1 B2} (RA1 : [Γ ||-<l1> A ≅ B1]) (RA2 : [Γ ||-<l2> A ≅ B2]) :=
-    forall t u, [Γ ||-<l1> t ≅ u : _ | RA1] <≈> [Γ ||-<l2> t ≅ u : _ | RA2].
+  Definition cumImpl l := forall Γ A B, [LogRel@{i j k l} l | Γ ||- A ≅ B] -> [LogRel@{i' j' k' l'} l | Γ ||- A ≅ B].
+  Definition cum l := forall Γ A B, [LogRel@{i j k l} l | Γ ||- A ≅ B] <≈> [LogRel@{i' j' k' l'} l | Γ ||- A ≅ B].
 
-  Let irrImpl {Γ l1 l2 A B1 B2} (RA1 : [Γ ||-<l1> A ≅ B1]) (RA2 : [Γ ||-<l2> A ≅ B2]) :=
-    forall t u, [Γ ||-<l1> t ≅ u : _ | RA1] -> [Γ ||-<l2> t ≅ u : _ | RA2].
+  Definition irr {Γ l1 l2 A B1 B2} (RA1 : [Γ ||-<l1> A ≅ B1]) (RA2 : [Γ ||-<l2> A ≅ B2]) :=
+    forall t u, [LogRel@{i j k l} l1 | Γ ||- t ≅ u : _ | RA1] <≈> [LogRel@{i' j' k' l'} l2 | Γ ||- t ≅ u : _ | RA2].
 
-  Lemma irrImplU {l1 l2} {Γ A B1 B2} (h : [Γ ||-U<l1> A ≅ B1]) (h' : [Γ ||-U<l2> A ≅ B2]) : irrImpl (LRU_ h) (LRU_ h').
+  End Defs.
+
+  Lemma irrImplU@{h i j k l h' i' j' k' l' } {l1 l2}
+    (ih : forall l, l << l1 -> l << l2 -> cumImpl@{h i j k h' i' j' k'} l)
+    {Γ A B1 B2} (h : [Γ ||-U<l1> A ≅ B1]) (h' : [Γ ||-U<l2> A ≅ B2]) {t u} :
+    [LogRel@{i j k l} l1 | _ ||- t ≅ u : _ | LRU_ h] -> [LogRel@{i' j' k' l'} l2 | _ ||- t ≅ u : _| LRU_ h'].
   Proof.
     assert (eq : h.(URedTy.level) = h'.(URedTy.level)) by now destruct h.(URedTy.lt), h'.(URedTy.lt).
-    cbn ; intros ?? [].
+    cbn ; intros [].
     eapply redTyRecFwd in relEq.
     unshelve econstructor.
     4: eapply redTyRecBwd.
-    all: destruct h, h'; cbn in *; subst; tea; cbn.
+    1-3: destruct h, h'; cbn in *; subst; tea; cbn.
+    eapply ih ; [|eapply URedTy.lt|].
+    all: rewrite <-eq; tea; eapply URedTy.lt.
   Qed.
 
-  Lemma irrU {l1 l2} {Γ A B1 B2} (h : [Γ ||-U<l1> A ≅ B1]) (h' : [Γ ||-U<l2> A ≅ B2]) : irr (LRU_ h) (LRU_ h').
-  Proof. intros ??; split; eapply irrImplU. Qed.
+
+  Universe i j k l i' j' k' l'.
+
+  Let irr {Γ l1 l2 A B1 B2} (RA1 : [Γ ||-<l1> A ≅ B1]) (RA2 : [Γ ||-<l2> A ≅ B2]) :=
+    Eval unfold irr in irr@{i j k l i' j' k' l'} RA1 RA2.
+
+  Lemma irrU@{h h'} {l1 l2}
+    (ih : forall l, l << l1 -> l << l2 -> cum@{h i j k h' i' j' k'} l)
+    {Γ A B1 B2} (h : [Γ ||-U<l1> A ≅ B1]) (h' : [Γ ||-U<l2> A ≅ B2]) : irr (LRU_ h) (LRU_ h').
+  Proof.
+    intros ??; split; eapply irrImplU;
+    intros ? lt1 lt2 ???; [apply (fst (ih _ lt1 lt2 _ _ _) ) | apply (snd (ih _ lt2 lt1 _ _ _) )].
+  Qed.
 
   Section IrrΠ.
   Context {l1 l2 Γ A B1 B2} (ΠA: [Γ ||-Π< l1 > A ≅ B1]) (ΠA': [Γ ||-Π< l2 > A ≅ B2])
@@ -134,853 +158,107 @@ Section Irrelevance.
   End IrrId.
 
 
-  Theorem irrLR {l1 l2}
+  Lemma irrLR_rec@{h h'}
+    {l1 l2}
+    (ih : forall l, l << l1 -> l << l2 -> cum@{h i j k h' i' j' k'} l)
     {Γ A B1 B2} (R1 : [Γ ||-<l1> A ≅ B1]) (R2 : [Γ ||-<l2> A ≅ B2]) : irr R1 R2.
   Proof.
     pose (i := invLREqL_whred R1 R2).
-    revert B2 R2 i; indLR R1.
-    - intros h B2 R2 [h']; subst; eapply irrU.
-    - intros neA ?? [neB [? eq]]; subst; intros ??; split; cbn.
+    revert B2 R2 i ih; indLR R1.
+    - intros h B2 R2 [h'] ih; subst; now eapply irrU.
+    - intros neA ?? [neB [? eq]] _; subst; intros ??; split; cbn.
       + intros []; econstructor; now rewrite eq.
       + intros [??]; econstructor; now rewrite eq in *.
-    - intros ΠA ihdom ihcod ?? [ΠA' [? eqdom eqcod]]; subst; cbn in *.
+    - intros ΠA ihdom ihcod ?? [ΠA' [? eqdom eqcod]] ?; subst; cbn in *.
       now eapply irrΠ.
-    - intros NA ?? [NA' ?]; subst; intros ??; split; now cbn.
-    - intros EA ?? [EA' ?]; subst; intros ??; split; now cbn.
-    - intros ΣA ihdom ihcod ?? [ΣA' [? eqdom eqcod]]; subst; cbn in *.
+    - intros NA ?? [NA' ?] ?; subst; intros ??; split; now cbn.
+    - intros EA ?? [EA' ?] ?; subst; intros ??; split; now cbn.
+    - intros ΣA ihdom ihcod ?? [ΣA' [? eqdom eqcod]] ?; subst; cbn in *.
       now eapply irrΣ.
-    - intros IA ih ihkr ?? [IA' [? eqty eqlhs eqrhs]]; subst.
+    - intros IA ih ?? [IA' [? eqty eqlhs eqrhs]] ?; subst.
       now eapply irrId.
   Qed.
 
+
+#[local]
+Lemma cumPolyRed@{h h'} {lA}
+  (ih : forall l, l << lA -> cum@{h i j k h' i' j' k'} l)
+  (Γ : context) (shp shp' pos pos' : term)
+  (PA : PolyRed@{i j k l} Γ lA shp shp' pos pos')
+  (IHshp : forall (Δ : context) (ρ : Δ ≤ Γ), [ |-[ ta ] Δ] ->
+    [LogRel@{i' j' k' l'} lA | Δ ||- shp⟨ρ⟩ ≅ shp'⟨ρ⟩])
+  (IHpos : forall (Δ : context) (a b : term) (ρ : Δ ≤ Γ) (h : [ |-[ ta ] Δ]),
+          [PolyRed.shpRed PA ρ h | _ ||- a ≅ b : _] ->
+          [LogRel@{i' j' k' l'} lA | Δ ||- pos[a .: ρ >> tRel] ≅ pos'[b .: ρ >> tRel]]) :
+  PolyRed@{i' j' k' l'} Γ lA shp shp' pos pos'.
+Proof.
+  unshelve econstructor.
+  + intros ; now eapply IHshp.
+  + intros; cbn; unshelve eapply IHpos; tea; now eapply irrLR_rec.
+Qed.
+
+
+Lemma cumLR_rec@{h h'} {lA}
+  (ih : forall l, l << lA -> cum@{h i j k h' i' j' k'} l)
+  {Γ A B} (lr : [ LogRel@{i j k l} lA | Γ ||- A ≅ B ]) :
+  [ LogRel@{i' j' k' l'} lA | Γ ||- A ≅ B ].
+Proof.
+  revert ih; indLR lr.
+  - intros [] ? ; eapply LRU_; now econstructor.
+  - intros; now eapply LRne_.
+  - intros [] IHdom IHcod ?; cbn in *.
+    eapply LRPi'; econstructor.
+    5: now eapply cumPolyRed.
+    all: tea.
+  - intros; now eapply LRNat_.
+  - intros; now eapply LREmpty_.
+  - intros [] IHdom IHcod ?; cbn in *.
+    eapply LRSig'; econstructor.
+    5: now eapply cumPolyRed.
+    all: tea.
+  - intros [] IHPar ?; cbn in *.
+    eapply LRId'; unshelve econstructor.
+    8-10: tea.
+    1: now eapply IHPar.
+    1,2: now apply  (irrLR_rec (fun l lt _ => ih l lt) tyRed).
+    constructor.
+    + intros ?? ?%(irrLR_rec (fun l lt _ => ih l lt) tyRed).
+      apply (irrLR_rec (fun l lt _ => ih l lt) tyRed); now symmetry.
+    + intros ??? ?%(irrLR_rec (fun l lt _ => ih l lt) tyRed) ?%(irrLR_rec (fun l lt _ => ih l lt) tyRed).
+      apply (irrLR_rec (fun l lt _ => ih l lt) tyRed); now etransitivity.
+Qed.
+
 End Irrelevance.
 
-
-
-Section Symmetry.
-  Context `{GenericTypingProperties}.
-
-  Universe v.
-
-  Notation "A <≈> B" := (prod@{v v} (A -> B) (B -> A)) (at level 90).
-
-  Record sym {Γ l A B} {R : [Γ ||-<l> A ≅ B]} :=
-    { symRed : [Γ ||-<l> B ≅ A] ;
-      symRedTm : forall {t u}, [Γ ||-<l> t ≅ u : _ | symRed] <≈> [Γ ||-<l> u ≅ t : _ | R] }.
-
-  Arguments sym : clear implicits.
-  Arguments sym {_ _ _ _}.
-
-  Definition symPoly {Γ l A A' B B'} (ΠA : PolyRed Γ l A A' B B')
-    (ihdom: forall (Δ : context) (ρ : Δ ≤ Γ) (h : [ |-[ ta ] Δ]), sym (PolyRed.shpRed ΠA ρ h))
-    (ihcod: forall (Δ : context) (a b : term) (ρ : Δ ≤ Γ) (h : [ |-[ ta ] Δ])
-      (ha : [PolyRed.shpRed ΠA ρ h | Δ ||- a ≅ b : _]), sym (PolyRed.posRed ΠA ρ h ha))
-      : PolyRed Γ l A' A B' B.
-  Proof.
-    unshelve econstructor.
-    * intros; now unshelve eapply symRed, ihdom.
-    * intros; (unshelve eapply symRed, ihcod); tea.
-      now eapply symRedTm.
-  Defined.
-
-  Definition symParamRedTy {T Γ l A A'} (ΠA : ParamRedTy T Γ l A A')
-    (ihdom: forall (Δ : context) (ρ : Δ ≤ Γ) (h : [ |-[ ta ] Δ]), sym (PolyRed.shpRed ΠA ρ h))
-    (ihcod: forall (Δ : context) (a b : term) (ρ : Δ ≤ Γ) (h : [ |-[ ta ] Δ])
-      (ha : [PolyRed.shpRed ΠA ρ h | Δ ||- a ≅ b : _]), sym (PolyRed.posRed ΠA ρ h ha))
-      : ParamRedTy T Γ l A' A.
-  Proof.
-    destruct ΠA; cbn in *; unshelve econstructor.
-    5,6: eassumption.
-    1,2: now symmetry.
-    now eapply symPoly.
-  Defined.
-
-  Section SymΠ.
-    Context {Γ l A A'} (ΠA : [Γ ||-Π<l> A ≅ A'])
-      (ihdom: forall (Δ : context) (ρ : Δ ≤ Γ) (h : [ |-[ ta ] Δ]), sym (PolyRed.shpRed ΠA ρ h))
-      (ihcod: forall (Δ : context) (a b : term) (ρ : Δ ≤ Γ) (h : [ |-[ ta ] Δ])
-        (ha : [PolyRed.shpRed ΠA ρ h | Δ ||- a ≅ b : _]), sym (PolyRed.posRed ΠA ρ h ha)).
-
-    Let symΠ := symParamRedTy ΠA ihdom ihcod.
-
-    Definition symIsLRFun {t} : isLRFun ΠA t <≈> isLRFun symΠ t.
-    Proof.
-      split.
-      - intros [???? Rbody|].
-        * constructor; tea.
-          1: etransitivity; tea; eapply ParamRedTy.eqdom.
-          intros; eapply ihcod, Rbody.
-        * constructor; eapply convneu_conv; tea; eapply ParamRedTy.eq.
-      - intros [???? Rbody|].
-        * constructor; tea.
-          1: etransitivity; tea; eapply ParamRedTy.eqdom.
-          intros ? a b ρ h ha.
-          unshelve eapply ihcod, irrLR, Rbody; tea.
-          now eapply ihdom.
-        * constructor; eapply convneu_conv; tea; eapply ParamRedTy.eq.
-    Qed.
-
-    Definition symPiRedTm {t} : PiRedTm ΠA t <≈> PiRedTm symΠ t.
-    Proof.
-      split; intros [?? ?%symIsLRFun]; econstructor; tea.
-      all: eapply redtmwf_conv; tea; apply ParamRedTy.eq.
-    Defined.
-
-    Definition symPiRedTmEq {t u} : PiRedTmEq ΠA t u <≈> PiRedTmEq symΠ u t.
-    Proof.
-      split; intros []; unshelve econstructor; try now eapply symPiRedTm.
-      1,3: cbn; eapply convtm_conv; [now symmetry| eapply PiRedTy.eq].
-      all: cbn; intros; unshelve eapply ihcod, irrLR, eqApp; tea; now eapply ihdom.
-    Qed.
-
-    Definition symLRΠ : sym (LRPi' ΠA).
-    Proof. exists (LRPi' symΠ); intros; cbn; split; eapply symPiRedTmEq. Qed.
-  End SymΠ.
-
-
-  Lemma symNe {Γ A B} : [Γ ||-ne A ≅ B] -> [Γ ||-ne B ≅ A].
-  Proof.
-    intros []; unshelve econstructor.
-    3,4: tea.
-    now symmetry.
-  Defined.
-
-  Lemma symNeNf {Γ t u A} : [Γ ||-NeNf t ≅ u : A] -> [Γ ||-NeNf u ≅ t : A].
-  Proof.
-    intros []; econstructor; tea; now symmetry.
-  Qed.
-
-  Lemma symNatRedTmEq {Γ} :
-    (forall t u, NatRedTmEq Γ t u -> NatRedTmEq Γ u t) ×
-    (forall t u, NatPropEq Γ t u -> NatPropEq Γ u t).
-  Proof.
-    eapply NatRedEqInduction.
-    - intros; econstructor; tea; now symmetry.
-    - constructor.
-    - intros; now constructor.
-    - intros; constructor; now eapply symNeNf.
-  Qed.
-
-  Lemma eq_subst_scons {Γ} a B : B[a..] = B[a⟨@wk_id Γ⟩ .: @wk_id Γ >> tRel].
-  Proof. now bsimpl. Qed.
-
-
-  Section SymΣ.
-    Context {Γ l A A'} (ΣA : [Γ ||-Σ<l> A ≅ A'])
-      (ihdom: forall (Δ : context) (ρ : Δ ≤ Γ) (h : [ |-[ ta ] Δ]), sym (PolyRed.shpRed ΣA ρ h))
-      (ihcod: forall (Δ : context) (a b : term) (ρ : Δ ≤ Γ) (h : [ |-[ ta ] Δ])
-        (ha : [PolyRed.shpRed ΣA ρ h | Δ ||- a ≅ b : _]), sym (PolyRed.posRed ΣA ρ h ha)).
-
-    Let symΣ := symParamRedTy ΣA ihdom ihcod.
-
-    Definition symIsLRPair {t} : isLRPair ΣA t <≈> isLRPair symΣ t.
-    Proof.
-      split.
-      - intros [???????? r1 r2|].
-        * unshelve eapply PairLRPair; tea.
-          2: etransitivity; tea; eapply ParamRedTy.eqdom.
-          + intros; now eapply ihdom.
-          + etransitivity; tea; erewrite 2!eq_subst_scons.
-            symmetry; eapply escapeEq.
-            unshelve eapply PolyRed.posRed, r1; gtyping.
-          + intros; (unshelve now eapply ihcod, irrLR); tea.
-        * constructor; eapply convneu_conv; tea; eapply ParamRedTy.eq.
-      - intros [???????? r1 r2|].
-        * unshelve eapply PairLRPair; tea.
-          2: etransitivity; tea; eapply ParamRedTy.eqdom.
-          + intros; now eapply ihdom.
-          + etransitivity; tea; erewrite 2!eq_subst_scons.
-            symmetry; eapply escapeEq.
-            unshelve eapply PolyRed.posRed, r1; gtyping.
-          + intros; (unshelve now eapply ihcod, irrLR); tea.
-        * constructor; eapply convneu_conv; tea; eapply ParamRedTy.eq.
-    Qed.
-
-    Definition symSigRedTm {t} : SigRedTm ΣA t <≈> SigRedTm symΣ t.
-    Proof.
-      split; intros [?? ?%symIsLRPair]; econstructor; tea.
-      all: eapply redtmwf_conv; tea; apply ParamRedTy.eq.
-    Defined.
-
-    Definition symSigRedTmEq {t u} : SigRedTmEq ΣA t u <≈> SigRedTmEq symΣ u t.
-    Proof.
-      split; intros []; unshelve econstructor; try now eapply symSigRedTm.
-      3,5: cbn; eapply convtm_conv; [now symmetry| eapply PiRedTy.eq].
-      1,2: cbn; intros; now eapply ihdom.
-      all: cbn; intros; unshelve (now eapply ihcod, irrLR); tea.
-    Qed.
-
-    Definition symLRΣ : sym (LRSig' ΣA).
-    Proof. exists (LRSig' symΣ); intros; cbn; split; eapply symSigRedTmEq. Qed.
-  End SymΣ.
-
-  Section SymId.
-  Context {Γ l A B} (IA: [Γ ||-Id< l > A ≅ B])
-    (ihdom:  sym (IdRedTy.tyRed IA))
-    (ihkr: forall (Δ : context) (ρ : Δ ≤ Γ) (wfΔ : [ |-[ ta ] Δ]), sym (IdRedTy.tyKripke IA ρ wfΔ)).
-
-  Lemma symId : [Γ ||-Id<l> B ≅ A].
-  Proof.
-    destruct IA; unshelve econstructor.
-    9,10: tea.
-    * now eapply ihdom.
-    * intros; now eapply ihkr.
-    * now symmetry.
-    * now eapply ihdom.
-    * now eapply ihdom.
-    * constructor.
-      1: intros ?? ?%ihdom; eapply ihdom; cbn in *; now symmetry.
-      intros ??? ?%ihdom ?%ihdom; eapply ihdom; cbn in *; now etransitivity.
-    * intros * ? ?%ihkr; eapply ihkr; cbn in *; now eapply tyKripkeTmEq.
-  Defined.
-
-  #[local] Instance : PER _ := IA.(IdRedTy.tyPER).
-  #[local] Instance : PER _ := symId.(IdRedTy.tyPER).
-
-  Lemma symIdPropEq {t u} : IdPropEq IA t u <≈> IdPropEq symId u t.
-  Proof.
-    pose proof (escapeEq (IA.(IdRedTy.tyRed))).
-    split; intros []; constructor; tea.
-    - etransitivity; tea; now symmetry.
-    - etransitivity; tea; now symmetry.
-    - eapply ihdom; etransitivity;[| eapply IdRedTy.lhsRed]; now symmetry.
-    - eapply ihdom; etransitivity;[| eapply IdRedTy.lhsRed]; now symmetry.
-    - eapply ihdom; etransitivity;[| eapply IdRedTy.rhsRed]; now symmetry.
-    - eapply ihdom; etransitivity;[| eapply IdRedTy.rhsRed]; now symmetry.
-    - eapply symNeNf, NeNf.conv_; tea; eapply IdRedTy.eq.
-    - etransitivity; tea.
-    - etransitivity; tea.
-    - eapply ihdom; etransitivity; [|apply symId.(IdRedTy.lhsRed)]; now symmetry.
-    - eapply ihdom; etransitivity;[| apply symId.(IdRedTy.lhsRed)]; now symmetry.
-    - eapply ihdom; etransitivity;[| apply symId.(IdRedTy.rhsRed)]; now symmetry.
-    - eapply ihdom; etransitivity;[| apply symId.(IdRedTy.rhsRed)]; now symmetry.
-    - eapply symNeNf, NeNf.conv_; tea; eapply IdRedTy.eq.
-  Qed.
-
-  Lemma symIdRedTmEq {t u} : IdRedTmEq IA t u <≈> IdRedTmEq symId u t.
-  Proof.
-    split; intros [????? ?%symIdPropEq]; econstructor; tea.
-    3,6: eapply convtm_conv; [now symmetry|]; eapply IdRedTy.eq.
-    all: eapply redtmwf_conv; tea; eapply IdRedTy.eq.
-  Qed.
-
-  Lemma symLRId : sym (LRId' IA).
-  Proof.
-    exists (LRId' symId).
-    intros; split; eapply symIdRedTmEq.
-  Qed.
-
-  End SymId.
-
-
-  Theorem symLR_rec {l}
-    (ih : forall l', l' << l -> forall {Γ A B} (R : [Γ ||-<l'> A ≅ B]), sym R)
-    {Γ A B} (R : [Γ ||-<l> A ≅ B]) : sym R.
-  Proof.
-    revert ih; indLR R.
-    - intros h ih; unshelve econstructor.
-      + destruct h; apply LRU_; now unshelve econstructor.
-      + cbn; intros ??; split; intros []; cbn in *.
-        all: unshelve econstructor; tea;[now symmetry|]; cbn.
-        1,2: eapply redTyRecBwd.
-        1,2: unshelve eapply symRed, ih, URedTy.lt.
-        1,2: now eapply redTyRecFwd.
-    - intros h _ ; unshelve econstructor.
-      1: now eapply LRne_, symNe.
-      + pose proof (convty_term (convtm_convneu UnivPos (neRedTy.eq h))).
-        cbn; intros ??; split; intros []; cbn in *.
-        all: unshelve econstructor; cbn.
-        5,6,8,9: eapply redtmwf_conv;tea; now symmetry.
-        1,2: eapply convneu_conv; [now symmetry|]; tea; now symmetry.
-    - intros ΠA ihdom ihcod ih.
-      eapply symLRΠ.
-      all: intros; eauto.
-    - intros NA _; unshelve econstructor.
-      + eapply LRNat_; destruct NA; now econstructor.
-      + intros; cbn; split; eapply symNatRedTmEq.
-    - intros EA _; unshelve econstructor.
-      + eapply LREmpty_; destruct EA; now econstructor.
-      + intro; cbn; split; intros []; econstructor; tea; now eapply symNeNf.
-    - intros ΣA ihdom ihcod ih; eapply symLRΣ; intros; eauto.
-    - intros IA ihdom ihkr ih; eapply symLRId; eauto.
-  Qed.
-
-  (* Universe Issue with ltInd.. should be fixable *)
-  (* Theorem symLR : forall {l Γ A B} (R : [Γ ||-<l> A ≅ B]), sym R.
-  Proof.  intros l. pattern l. eapply ltInd. intros; eapply symLR_rec; intros; eapply X. eapply (ltInd _ l). refine (ltInd _ (@symLR_rec)). *)
-
-  Theorem symLR0 : forall {Γ A B} (R : [Γ ||-<zero> A ≅ B]), sym R.
-  Proof.
-    eapply symLR_rec; intros ? h; inversion h.
-  Qed.
-
-  Theorem symLR : forall {l Γ  A B} (R : [Γ ||-<l> A ≅ B]), sym R.
-  Proof.
-    intros []; [intros; eapply symLR0| apply symLR_rec].
-    intros ? h; inversion h; intros; eapply symLR0.
-  Qed.
-
-End Symmetry.
+Lemma cumLR0@{i j k l i' j' k' l' v} `{GenericTypingProperties} :
+  cum@{v i j k l i' j' k' l'} zero.
+Proof.
+  intros; split; eapply cumLR_rec;
+  intros ? h; inversion h.
+Qed.
 
 
 
+Theorem irrLR@{i j k l i' j' k' l' v} `{GenericTypingProperties} {l1 l2}
+  {Γ A B1 B2} (R1 : [Γ ||-<l1> A ≅ B1]) (R2 : [Γ ||-<l2> A ≅ B2]) :
+    irr@{v i j k l i' j' k' l'} R1 R2.
+Proof.
+  split; eapply irrLR_rec; intros l [] ?; exact cumLR0.
+Qed.
+
+Theorem cumLR@{i j k l i' j' k' l'} `{GenericTypingProperties} {lA}
+  {Γ A B} (lr : [ LogRel@{i j k l} lA | Γ ||- A ≅ B ]) :
+  [ LogRel@{i' j' k' l'} lA | Γ ||- A ≅ B ].
+Proof.
+  eapply cumLR_rec; tea; intros ? []; exact cumLR0.
+Qed.
 
 
 
-(** We show a general version of irrelevance, saying that if A and A' are reducible (at levels logical relation levels lA, lA')
-and A' is reducibly convertible to A, then the reducibility predicates they decode to are equivalent.
-From this, both a simpler version of irrelevance and symmetry follow, by using reflexivity
-in the right places. *)
-(** Interestingly, we also show irrelevance with respect to universe levels, which is crucial
-in later parts of the development, where this avoids creating spurious constraints on universe levels.*)
-
+(*
 Lemma subst_wk_id_tail Γ P t : P[t .: @wk_id Γ >> tRel] = P[t..].
 Proof. setoid_rewrite id_ren; now bsimpl. Qed.
 
-
-Section Irrelevances.
-Context `{GenericTypingProperties}.
-
-Section EquivLR.
-  Universe j k j' k' v.
-
-  Notation "A <≈> B" := (prod@{v v} (A -> B) (B -> A)) (at level 90).
-
-  Record equivLR {kA : RedRel@{j k}} {kA' : RedRel@{j' k'}} {Γ A A'} := {
-    lrConvL : forall C, [kA | Γ ||- A ≅ C] <≈> [kA' | Γ ||- A' ≅ C] ;
-    lrConvR : forall C, [kA | Γ ||- C ≅ A] <≈> [kA' | Γ ||- C ≅ A'] ;
-    lrTmL : forall C C' t u (RA : [kA | Γ ||- A ≅ C]) (RA' : [kA' | Γ ||- A' ≅ C']),
-      [RA | _ ||- t ≅ u : _] <≈> [RA' | _ ||- t ≅ u : _] ;
-    lrTmR : forall C C' t u (RA : [kA | Γ ||- C ≅ A]) (RA' : [kA' | Γ ||- C' ≅ A']),
-      [RA | _ ||- t ≅ u : _] <≈> [RA' | _ ||- t ≅ u : _] ;
-  }.
-
-End EquivLR.
-
-Arguments equivLR : clear implicits.
-
-Record implLR@{j k j' k'} {kA : RedRel@{j k}} {kA' : RedRel@{j' k'}} {Γ A A'} := {
-    ilrConvL : forall C, [kA | Γ ||- A ≅ C] -> [kA' | Γ ||- A' ≅ C] ;
-    ilrConvR : forall C, [kA | Γ ||- C ≅ A] -> [kA' | Γ ||- C ≅ A'] ;
-    ilrTmL : forall C C' t u (RA : [kA | Γ ||- A ≅ C]) (RA' : [kA' | Γ ||- A' ≅ C']),
-      [RA | _ ||- t ≅ u : _] -> [RA' | _ ||- t ≅ u : _] ;
-    ilrTmR : forall C C' t u (RA : [kA | Γ ||- C ≅ A]) (RA' : [kA' | Γ ||- C' ≅ A']),
-      [RA | _ ||- t ≅ u : _] -> [RA' | _ ||- t ≅ u : _] ;
-}.
-Arguments implLR : clear implicits.
-
-Lemma impl_equivLR@{j k j' k' v} (kA : RedRel@{j k}) (kA' : RedRel@{j' k'}) Γ A A' :
-  implLR@{j k j' k'} kA kA' Γ A A' -> implLR@{j' k' j k} kA' kA Γ A' A ->
-  equivLR@{j k j' k' v} kA kA' Γ A A'.
-Proof.
-  intros [] []; constructor; intros; split; eauto.
-Defined.
-
-Lemma equiv_implLR1@{j k j' k' v} (kA : RedRel@{j k}) (kA' : RedRel@{j' k'}) Γ A A' :
-  equivLR@{j k j' k' v} kA kA' Γ A A' ->
-  implLR@{j k j' k'} kA kA' Γ A A'.
-Proof.
-  intros e; constructor; intros.
-  - edestruct e as [[]]; eauto.
-  - edestruct e as [? []]; eauto.
-  - edestruct e as [?? []]; eauto.
-  - edestruct e as [??? []]; eauto.
-Defined.
-
-Lemma equiv_implLR2@{j k j' k' v} (kA : RedRel@{j k}) (kA' : RedRel@{j' k'}) Γ A A' :
-  equivLR@{j k j' k' v} kA kA' Γ A A' ->
-  implLR@{j' k' j k} kA' kA Γ A' A.
-Proof.
-  intros e; constructor; intros.
-  - edestruct e as [[]]; eauto.
-  - edestruct e as [? []]; eauto.
-  - edestruct e as [?? []]; eauto.
-  - edestruct e as [??? []]; eauto.
-Defined.
-
-
-Lemma transImplLR@{j k j' k' j'' k''} kA kA' kA'' Γ A A' A''
-  (h : implLR@{j k j' k'} kA kA' Γ A A')
-  (h' : implLR@{j' k' j'' k''} kA' kA'' Γ A' A'') :
-  implLR@{j k j'' k''} kA kA'' Γ A A''.
-Proof.
-  constructor; intros.
-  - do 2 (eapply ilrConvL; tea).
-  - do 2 (eapply ilrConvR; tea).
-  - unshelve (do 2 (eapply ilrTmL; tea)).
-    2: now eapply ilrConvL.
-  - unshelve (do 2 (eapply ilrTmR; tea)).
-    2: now eapply ilrConvR.
-Qed.
-
-
-
-Lemma ureflConvEquivLR@{j k j' k' v} (kA : RedRel@{j k}) (kA' : RedRel@{j' k'}) Γ A A'
-  (RAA' : [kA | Γ ||- A ≅ A'])
-  (h : equivLR@{j k j' k' v} kA kA' Γ A A') : [kA' | Γ ||- A' ≅ A'].
-Proof. now eapply h.(lrConvL). Qed.
-
-Lemma lreflConvEquivLR@{j k j' k' v} (kA : RedRel@{j k}) (kA' : RedRel@{j' k'}) Γ A A'
-  (RAA' : [kA | Γ ||- A ≅ A'])
-  (h : equivLR@{j k j' k' v} kA' kA Γ A A') : [kA' | Γ ||- A ≅ A].
-Proof. now eapply h.(lrConvR). Qed.
-
-Lemma symConvEquivLR@{j k j' k' v} (kA : RedRel@{j k}) (kA' : RedRel@{j' k'}) Γ A A'
-  (RAA' : [kA | Γ ||- A ≅ A'])
-  (h : equivLR@{j k j' k' v} kA kA' Γ A A') :
-  [kA | Γ ||- A' ≅ A].
-Proof. now eapply h.(lrConvR), ureflConvEquivLR. Qed.
-
-Lemma symConvEquivLR'@{j k j' k' v} (kA : RedRel@{j k}) (kA' : RedRel@{j' k'}) Γ A A'
-  (RAA' : [kA | Γ ||- A ≅ A'])
-  (h : equivLR@{j k j' k' v} kA' kA Γ A A') :
-  [kA | Γ ||- A' ≅ A].
-Proof. now eapply h.(lrConvL), lreflConvEquivLR. Qed.
-
-Lemma symEquivLR@{j k j' k' v} (kA : RedRel@{j k}) (kA' : RedRel@{j' k'}) Γ A A' :
-  equivLR@{j k j' k' v} kA kA' Γ A A' -> equivLR@{j' k' j k v} kA' kA Γ A' A.
-Proof.
-  intros h. eapply impl_equivLR;
-   [now apply equiv_implLR2| now apply equiv_implLR1].
-Qed.
-
-Lemma transEquivLR@{j k j' k' j'' k'' v} kA kA' kA'' Γ A A' A''
-  (h : equivLR@{j k j' k' v} kA kA' Γ A A')
-  (h' : equivLR@{j' k' j'' k'' v} kA' kA'' Γ A' A'') :
-  equivLR@{j k j'' k'' v} kA kA'' Γ A A''.
-Proof.
-  eapply impl_equivLR; eapply transImplLR; first [now eapply equiv_implLR1| now eapply equiv_implLR2].
-Qed.
-
-Notation "[ R | Γ ||-≅]" := (fun A B  => [R | Γ ||- A ≅ B]) (R at level 50).
-
-
-Lemma convEquivLRSym@{j k j' k' v} k k' Γ
-  (h : forall A B, [k | Γ ||- A ≅ B] -> equivLR@{j k j' k' v} k k' Γ A B) :
-  Symmetric@{Set v} ([k | Γ ||-≅]).
-Proof.
-  intros A B RAB; eapply symConvEquivLR; tea; now apply h.
-Qed.
-
-Lemma convEquivLRSym'@{j k j' k' v} k k' Γ
-  (h : forall A B, [k' | Γ ||- A ≅ B] -> equivLR@{j k j' k' v} k k' Γ A B) :
-  Symmetric@{Set v} ([k' | Γ ||-≅]).
-Proof.
-  intros A B RAB; eapply symConvEquivLR'; tea; now apply h.
-Qed.
-
-Lemma convEquivLRDiag@{j k j' k' v} k k' Γ
-  (h : forall A B, [k | Γ ||- A ≅ B] -> equivLR@{j k j' k' v} k k' Γ A B)
-  (h' : forall A B, [k' | Γ ||- A ≅ B] -> equivLR@{j k j' k' v} k k' Γ A B) :
-  forall A B, [k | Γ ||- A ≅ B] -> equivLR@{j k j k v} k k Γ A B.
-Proof.
-  intros ?? R.
-  eapply transEquivLR.
-  1: now apply h.
-  apply symEquivLR.
-  apply h'; eapply ureflConvEquivLR; tea; eauto.
-Qed.
-
-Lemma convEquivLRDiag'@{j k j' k' v} k k' Γ
-  (h : forall A B, [k | Γ ||- A ≅ B] -> equivLR@{j k j' k' v} k k' Γ A B)
-  (h' : forall A B, [k' | Γ ||- A ≅ B] -> equivLR@{j k j' k' v} k k' Γ A B) :
-  forall A B, [k' | Γ ||- A ≅ B] -> equivLR@{j k j k v} k' k' Γ A B.
-Proof.
-  pose proof (convEquivLRSym' _ _ _ h').
-  intros ?? R. eapply (symmetry (R:=[k' | Γ ||-≅])) in R.
-  eapply transEquivLR; eapply symEquivLR.
-  1: now eapply h'.
-  apply symEquivLR.
-  apply h ; eapply lreflConvEquivLR; tea; eauto.
-Qed.
-
-
-Lemma convEquivLRDiagPER@{j k v} k Γ  (h : forall A B, [k | Γ ||- A ≅ B] -> equivLR@{j k j k v} k k Γ A B) :
-  PER@{Set v} ([k | Γ ||-≅]).
-Proof.
-  constructor; [ now eapply convEquivLRSym |].
-  intros A B C RAB RBC; now eapply (h _ _ RAB).(lrConvL).
-Qed.
-
-Lemma convEquivLRPER@{j k j' k' v} k k' Γ
-  (h : forall A B, [k | Γ ||- A ≅ B] -> equivLR@{j k j' k' v} k k' Γ A B)
-  (h' : forall A B, [k' | Γ ||- A ≅ B] -> equivLR@{j k j' k' v} k k' Γ A B) :
-  PER@{Set v} ([k | Γ ||-≅]).
-Proof.
-  apply convEquivLRDiagPER; now eapply convEquivLRDiag.
-Qed.
-
-Lemma convEquivLRPER'@{j k j' k' v} k k' Γ
-  (h : forall A B, [k | Γ ||- A ≅ B] -> equivLR@{j k j' k' v} k k' Γ A B)
-  (h' : forall A B, [k' | Γ ||- A ≅ B] -> equivLR@{j k j' k' v} k k' Γ A B) :
-  PER@{Set v} ([k' | Γ ||-≅]).
-Proof.
-  apply convEquivLRDiagPER; now eapply convEquivLRDiag'.
-Qed.
-
-(* Lemma equivLR_irrTmL :
-    forall C C' t u (RA : [kA | Γ ||- A ≅ C]) (RA' : [kA' | Γ ||- C' ≅ A']),
-      [RA | _ ||- t ≅ u : _] <≈> [RA' | _ ||- t ≅ u : _] ; *)
-
-
-(* Section EquivLR.
-  Universe i j k l i' j' k' l' v.
-
-  Notation "A <≈> B" := (prod@{v v} (A -> B) (B -> A)) (at level 90).
-
-  Record equivLR {Γ lA A Γ' lA' A'} := {
-    lrConvL : forall C, [LogRel@{i j k l} lA | Γ ||- A ≅ C] <≈> [LogRel@{i' j' k' l'} lA' | Γ' ||- A' ≅ C] ;
-    lrConvR : forall C, [LogRel@{i j k l} lA | Γ ||- C ≅ A] <≈> [LogRel@{i' j' k' l'} lA' | Γ' ||- C ≅ A'] ;
-    lrTmL : forall C t u (RA : [LogRel@{i j k l} lA | Γ ||- A ≅ C]) (RA' : [LogRel@{i' j' k' l'} lA' | Γ' ||- A' ≅ C]),
-      [RA | _ ||- t ≅ u : _] <≈> [RA' | _ ||- t ≅ u : _] ;
-    lrTmR : forall C t u (RA : [LogRel@{i j k l} lA | Γ ||- C ≅ A]) (RA' : [LogRel@{i' j' k' l'} lA' | Γ' ||- C ≅ A']),
-      [RA | _ ||- t ≅ u : _] <≈> [RA' | _ ||- t ≅ u : _] ;
-  }.
-
-End EquivLR.
-
-Arguments equivLR : clear implicits.
-
-
-Lemma ureflConvEquivLR@{i j k l i' j' k' l' v} Γ lA A Γ' lA' A' (RAA' : [LogRel@{i j k l} lA | Γ ||- A ≅ A'])
-  (h : equivLR@{i j k l i' j' k' l' v} Γ lA A Γ' lA' A') : [LogRel@{i j k l} lA' | Γ' ||- A' ≅ A'].
-Proof. now eapply h.(lrConvL). Qed.
-
-Lemma symConvEquivLR@{i j k l i' j' k' l' v} Γ lA A Γ' lA' A' (RAA' : [LogRel@{i j k l} lA | Γ ||- A ≅ A'])
-  (h : equivLR@{i j k l i' j' k' l' v} Γ lA A Γ' lA' A') : [LogRel@{i j k l} lA | Γ ||- A' ≅ A].
-Proof. now eapply h.(lrConvR), ureflConvEquivLR. Qed.
-
-Lemma symEquivLR@{i j k l i' j' k' l' v} Γ lA A Γ' lA' A' (h : equivLR@{i j k l i' j' k' l' v} Γ lA A Γ' lA' A') :
-  equivLR@{ i' j' k' l' i j k l v}  Γ' lA' A' Γ lA A.
-Proof.
-  constructor; intros; split; try first [apply h.(lrConvL)|apply h.(lrConvR)| apply h.(lrTmL)| apply h.(lrTmR)].
-Qed.
-
-Lemma transEquivLR@{i j k l i' j' k' l' i'' j'' k'' l'' v} Γ lA A Γ' lA' A' Γ'' lA'' A''
-  (h : equivLR@{i j k l i' j' k' l' v} Γ lA A Γ' lA' A')
-  (h' : equivLR@{i' j' k' l' i'' j'' k'' l'' v} Γ' lA' A' Γ'' lA'' A'') :
-  equivLR@{i j k l i'' j'' k'' l'' v} Γ lA A Γ'' lA'' A''.
-Proof.
-  constructor; intros; split; intros;
-    try first [eapply h.(lrConvL)|eapply h.(lrConvR)| eapply h.(lrTmL)| eapply h.(lrTmR)];
-    try first [eapply h'.(lrConvL)|eapply h'.(lrConvR)| eapply h'.(lrTmL)| eapply h'.(lrTmR)]; tea;
-    try first [eapply h.(lrConvL)|eapply h.(lrConvR)| eapply h.(lrTmL)| eapply h.(lrTmR)]; tea.
-    Unshelve. all: now first [eapply h.(lrConvL)|eapply h.(lrConvR)].
-Qed.
-
-Lemma convEquivLRPER@{i j k l v} Γ l  (h : forall A B, [LogRel@{i j k l} l | Γ ||- A ≅ B] -> equivLR@{i j k l i j k l v} Γ l A Γ l B) :
-  PER@{Set l} (fun A B => [LogRel@{i j k l} l | Γ ||- A ≅ B]).
-Proof.
-  constructor.
-  - intros A B RAB; eapply symConvEquivLR; tea; now apply h.
-  - intros A B C RAB RBC; now eapply (h _ _ RAB).(lrConvL).
-Qed. *)
-
-Section NeIrrelevance.
-Import neRedTy.
-
-#[local]
-Instance nePER {Γ} : PER (neRedTy Γ).
-Proof.
-  constructor.
-  - intros ?? []; econstructor; tea; now symmetry.
-  - intros ??? Rxy Ryz.
-    pose proof (whredty_det _ _ (whredR Rxy) (whredL Ryz)).
-    destruct Rxy, Ryz; cbn in *; subst; econstructor; tea; now etransitivity.
-Qed.
-
-#[local]
-Instance neTmPER@{k} {Γ A B} (h : [Γ ||-ne A ≅ B]) : PER@{Set k} (fun t u=> neRedTmEq t u h).
-Proof.
-  constructor.
-  - intros ?? []; econstructor; tea; now symmetry.
-  - intros ??? Rxy Ryz.
-    pose proof (whredtm_det _ _ _ _ (neRedTmEq.whredR Rxy) (neRedTmEq.whredL Ryz)).
-    destruct Rxy, Ryz; cbn in *; subst; econstructor; tea; now etransitivity.
-Qed.
-
-
-Lemma neIrrelevanceImpl {Γ lA lB A B} : [Γ ||-ne A ≅ B] -> implLR (LogRel lA) (LogRel lB) Γ A B.
-Proof.
-  intros Rne; pose (RlA:= LRne_ lA Rne).
-  (* ; pose (RlB:= LRne_ lB (symmetry Rne)). *)
-  constructor.
-  - intros ? R ; pose proof (invLREqL_whred RlA R) as []; subst.
-    apply LRne_; etransitivity; tea; now symmetry.
-  - intros ? R ; pose proof (invLREqR_whred RlA R) as [] ; subst.
-    apply LRne_; now etransitivity.
-  - intros ???? RA RB.
-    pose proof (invLREqBothL_whred RlA RA RB) as [[RAne [->]] [RBne [->]]]; cbn in *.
-    assert ([Γ |- RAne.(tyL) ≅ RBne.(tyL)]).
-    1:{
-      replace RAne.(tyL) with Rne.(tyL); tea.
-      replace RBne.(tyL) with Rne.(tyR); tea.
-      destruct Rne; gtyping.
-    }
-    cbn; intros []; cbn; econstructor.
-    1,2: eapply redtmwf_conv; tea.
-    now eapply convneu_conv.
-  - intros ???? RA RB.
-    pose proof (invLREqBothR_whred RlA RA RB) as [[RAne [-> ?]] [RBne [-> ?]]].
-    assert ([Γ |- RAne.(tyL) ≅ RBne.(tyL)]).
-    1:{
-      destruct RAne, RBne, Rne; cbn in *; subst.
-      eapply convty_term, convtm_convneu.
-      1: constructor.
-      do 2 (etransitivity; tea); now symmetry.
-    }
-    cbn; intros []; cbn; econstructor.
-    1,2: eapply redtmwf_conv; tea.
-    now eapply convneu_conv.
-Qed.
-
-Lemma neIrrelevance {Γ lA lB A B} (h : [Γ ||-ne A ≅ B]) :
-  equivLR (LogRel lA) (LogRel lB) Γ A B.
-Proof.
-  eapply impl_equivLR; eapply neIrrelevanceImpl; tea; now symmetry.
-Qed.
-
-End NeIrrelevance.
-
-
-
-Section LRIrrelevant.
-Universe (*u *) v.
-(** u is a small universe level that may be instanciated to Set. v is a large universe level *)
-
-Notation "A <≈> B" := (prod@{v v} (A -> B) (B -> A)) (at level 90).
-
-Section LRIrrelevantInductionStep.
-
-Universe i j k l i' j' k' l'.
-
-
-#[local]
-Definition IHStatement lA lA' :=
-  forall l0 (ltA : l0 << lA) (ltA' : l0 << lA') Γ,
-    (forall A B, [LogRelRec@{i j k} lA l0 ltA | Γ ||- A ≅ B] ->
-      equivLR@{j k j' k' v} (LogRelRec@{i j k} lA l0 ltA) (LogRelRec@{i' j' k'} lA' l0 ltA') Γ A B)
-    × (forall A B, [LogRelRec@{i' j' k'} lA' l0 ltA' | Γ ||- A ≅ B] ->
-      equivLR@{j k j' k' v} (LogRelRec@{i j k} lA l0 ltA) (LogRelRec@{i' j' k'} lA' l0 ltA')  Γ A B).
-
-(* Lemma eqTmUPER {Γ A B lA lA'} (h: [Γ ||-U< lA > A ≅ B]) : IHStatement lA lA' ->
-  PER (fun t u : term => [LogRelRec lA | Γ ||-U t ≅ u : A ≅ B | h]).
-Proof.
-  destruct h as [l0 ltA]. cbn.
-  intros. split.
-  - intros ?? []; cbn in *. *)
-
-
-Definition IHCoroL {lA lA'} : IHStatement lA lA' ->
-  forall l0 (ltA : l0 << lA) (ltA' : l0 << lA') Γ A B,
-    [LogRelRec@{i j k} lA l0 ltA | Γ ||- A ≅ B] ->
-    equivLR@{j k j' k' v} (LogRelRec@{i j k} lA l0 ltA) (LogRelRec@{i' j' k'} lA' l0 ltA')  Γ A A.
-Proof.
-  intros ih l0 ltA ltA' Γ ?? RAB; specialize (ih l0 ltA ltA' Γ) as [e e'].
-  pose proof (convEquivLRPER _ _ _ e e').
-  apply e.
-  eapply (transitivity (R:=[LogRelRec@{i j k} lA l0 ltA|Γ||-≅])).
-  2: eapply (symmetry (R:=[LogRelRec@{i j k} lA l0 ltA|Γ||-≅])).
-  all: tea.
-Qed.
-
-Definition IHCoroR {lA lA'} : IHStatement lA lA' ->
-  forall l0 (ltA : l0 << lA) (ltA' : l0 << lA') Γ A B,
-    [LogRelRec@{i' j' k'} lA' l0 ltA' | Γ ||- A ≅ B] ->
-    equivLR@{j k j' k' v} (LogRelRec@{i j k} lA l0 ltA) (LogRelRec@{i' j' k'} lA' l0 ltA')  Γ A A.
-Proof.
-  intros ih l0 ltA ltA' Γ ?? RAB; specialize (ih l0 ltA ltA' Γ) as [e e'].
-  pose proof (convEquivLRPER' _ _ _ e e').
-  apply e'.
-  eapply (transitivity (R:=[LogRelRec@{i' j' k'} lA' l0 ltA'|Γ||-≅])).
-  2: eapply (symmetry (R:=[LogRelRec@{i' j' k'} lA' l0 ltA'|Γ||-≅])).
-  all: tea.
-Qed.
-
-
-#[local]
-Lemma UnivIrrelevanceLRPack
-  {Γ lA lB A A' B B'}
-  (IH : IHStatement lA lB)
-  (hUA : [Γ ||-U<lA> A ≅ A'])
-  (hUB : [Γ ||-U<lB> B ≅ B'])
-  (hAB : [Γ ||-U<lA> A ≅ B])
-  : equivLR@{k l k' l' v} (LogRel@{i j k l} lA) (LogRel@{i' j' k' l'} lB) Γ A B
-    × PER (fun t u : term => [LogRelRec lA | Γ ||-U t ≅ u : A ≅ B | hAB]).
-Proof.
-  pose (RA := LRU_ hUA).
-  pose (RB := LRU_ hUB).
-  pose proof (level_unique hUA hUB hAB).
-  pose proof (level_unique hAB hUB hAB).
-  destruct hUA as [? ltA], hUB as [? ltB]; cbn in *; subst.
-  split; [constructor|].
-  + intros; split; intros lr.
-    all: (destruct (invLR_whred RA lr) + destruct (invLR_whred RB lr)).
-    all: apply LRU_; subst; now econstructor.
-  + intros; split; intros lr.
-    all: (destruct (invLRr_whred RA lr) + destruct (invLRr_whred RB lr)).
-    all: apply LRU_; now econstructor.
-  + intros ?? T U RA' RB'.
-    pose proof (invLREqL_whred RA RA') as [hA']; subst.
-    pose proof (invLREqL_whred RB RB') as [hB']; subst.
-    pose proof (h := level_unique hA' hB' hAB); destruct hA' as [? lt1], hB' as [l1 lt2].
-    cbn in *; subst; split; intros []; unshelve econstructor; cbn in *; tea.
-    1: now apply (IHCoroL IH l1 lt1 lt2 Γ T U relEq).
-    now apply (IHCoroR IH l1 lt1 lt2 Γ T U relEq).
-  + intros ?? T U RA' RB'.
-    pose proof (invLREqR_whred RA RA') as [hA']; subst.
-    pose proof (invLREqR_whred RB RB') as [hB']; subst.
-    pose proof (h := level_unique' hA' hB' hAB); destruct hA' as [? lt1], hB' as [l1 lt2].
-    cbn in *; subst; split; intros []; unshelve econstructor; cbn in *; tea.
-    1: now apply (IHCoroL IH l1 lt1 lt2 Γ T U relEq).
-    now apply (IHCoroR IH l1 lt1 lt2 Γ T U relEq).
-  + specialize (IH _ (URedTy.lt hAB) ltB Γ) as [e e'].
-    pose proof (convEquivLRPER _ _ _ e e').
-    constructor.
-    * intros ?? []; econstructor.
-      1: now symmetry.
-      now eapply (@symmetry _ _ X.(PER_Symmetric)).
-    * intros ??? [? redR1] [redL2 ]; econstructor.
-      1: etransitivity; tea.
-      epose proof (h := whredtm_det _ _ _ _ (URedTm.whred redR1) (URedTm.whred redL2)).
-      now replace (URedTm.te redR1) with (URedTm.te redL2) by (symmetry ; apply h).
-      now eapply (@transitivity _ _ X.(PER_Transitive)).
-Qed.
-
-(** ** The main theorem *)
-
-#[local]
-Lemma LRconvEquiv {lA lB}
-  (IH : IHStatement lA lB)
-  (Γ : context) (A A' B B' : term)
-  (RA : [LogRel@{i j k l} lA | Γ ||- A ≅ A'])
-  (RB : [LogRel@{i' j' k' l'} lB | Γ ||- B ≅ B'])
-  (* {l} *)
-  (RAB : [LogRel@{i j k l} lA | Γ ||- A ≅ B]) :
-  (* (l = lA \/ l = lB) -> *)
-  equivLR (LogRel@{i j k l} lA) (LogRel@{i' j' k' l'} lB) Γ A B × PER (RAB.(LRPack.eqTm)).
-Proof.
-  revert (*lA*) lB A' RA B' RB IH; indLR RAB.
-  - intros; eapply UnivIrrelevanceLRPack; tea.
-    (* + unshelve eapply (invLR RA _ (whredR (LRU_ h))); cbn; destruct h; gtyping. *)
-    + unshelve eapply (invLR RB _ (whredR (LRU_ h))); cbn; destruct h; gtyping.
-  - intros neA **; split.
-    + now eapply neIrrelevance.
-    + now eapply neTmPER.
-  - intros ΠA ihdom ihcod **.
-    pose (R0 := LRPi' ΠA).
-    pose proof (invLREqBothL_whred R0 RA RB) as [[hA' []] [hB' []]]; subst; cbn in *.
-    unshelve epose proof (ihdom' := fun Δ ρ h => ihdom Δ ρ h (*lA*) lB (ParamRedTy.domR hA')⟨ρ⟩ _ (ParamRedTy.domR hB')⟨ρ⟩ _ IH).
-    1: rewrite <-e0; now eapply hA'.(PolyRed.shpRed).
-    1: rewrite <-e3; now eapply hB'.(PolyRed.shpRed).
-    unshelve epose proof (ihcod' := fun Δ a b ρ h Rab => ihcod Δ a b ρ h Rab (*lA*) lB (ParamRedTy.codR hA')[b .: ρ >> tRel] _ (ParamRedTy.codR hB')[b .: ρ >> tRel] _ IH).
-    1:{
-      rewrite <-e1; unshelve eapply hA'.(PolyRed.posRed); tea.
-      set (PolyRed.shpRed ΠA ρ h) in Rab.
-      set (PolyRed.shpRed hA' ρ h).
-      pose proof (e':= fst (ihdom' _ ρ h)).
-      pose proof (e := fst (ihdom' _ ρ h)).
-      rewrite <- e0 in e'.
-      unshelve eapply e'.(lrTmL).
-      2: now eapply e.(lrConvL).
-      eapply e.(lrTmL).
-      exact Rab.
-    }
-    1:{
-      rewrite <-e4; unshelve eapply hB'.(PolyRed.posRed); tea.
-      set (PolyRed.shpRed ΠA ρ h) in Rab.
-      set (PolyRed.shpRed hB' ρ h).
-      destruct (ihdom' _ ρ h) as [e domPER].
-      pose proof (e':= fst (ihdom' _ ρ h)).
-      rewrite <- e3 in e'.
-      unshelve eapply e'.(lrTmL).
-      2: eassumption.
-      unshelve eapply urefl. 2: eassumption.
-    }
-    admit.
-  - admit.
-  - admit.
-  - admit.
-  - admit.
-Admitted.
-
-#[local]
-Lemma IrrRec0 : IHStatement zero zero.
-Proof.
-  intros ? ltA; inversion ltA.
-Qed.
-
-(** Safety check: we did not add constraints we did not mean to *)
-Fail Fail Constraint i < i'.
-Fail Fail Constraint i' < i.
-Fail Fail Constraint j < j'.
-Fail Fail Constraint j' < j.
-Fail Fail Constraint k < k'.
-Fail Fail Constraint k' < k.
-Fail Fail Constraint l < l'.
-Fail Fail Constraint l' < l.
-
-End LRIrrelevantInductionStep.
-
-
-#[local]
-Theorem IrrRec@{i j k l i' j' k' l' v} {lA} {lA'} :
-  IHStatement@{i j k l i' j' k' l' v} lA lA'.
-Proof.
-  intros l0 ltA ltA'.
-  destruct ltA. destruct ltA'. cbn in *; intros.
-  split; intros ?? R; unshelve eapply (fst (LRconvEquiv IrrRec0 Γ A _ B A R _ R)).
-  - intros. eapply
-  - intros Γ t. split.
-    + eapply (LRIrrelevantCumTy@{u i j k u i' j' k'} IrrRec0@{u i j k u i' j' k'}).
-    + eapply (LRIrrelevantCumTy@{u i' j' k' u i j k} IrrRec0@{u i' j' k' u i j k}).
-  - intros Γ t lr1 lr2 u.
-    destruct (LRIrrelevantPreds@{u i j k u i' j' k'} IrrRec0@{u i j k u i' j' k'} Γ t t
-                (lr1 : LRPackAdequate (LogRel@{u i j k} zero) lr1)
-                (lr2 : LRPackAdequate (LogRel@{u i' j' k'} zero) lr2)
-                (reflLRTyEq lr1)) as [tyEq _].
-    exact (tyEq u).
-Qed.
-
-
-
-
-#[local]
-Lemma LRIrrelevantPreds {lA lB}
-  (IH : IHStatement lA lB)
-  (Γ : context) (A A' B B' : term)
-  (* (RA : [LogRel@{i j k l} lA | Γ ||- A ≅ A']) *)
-  (RB : [LogRel@{i' j' k' l'} lB | Γ ||- B ≅ B']) :
-  [LogRel@{i j k l} lA | Γ ||- A ≅ B] ->
-  equivLR (LogRel@{i j k l} lA) (LogRel@{i' j' k' l'} lB) Γ A B.
-Proof.
-  intros RAB; revert lB IH A' B' RB; indLR RAB.
-  - intros; eapply UnivIrrelevanceLRPack; tea.
-    unshelve eapply (invLR RB _ (whredR (LRU_ h))); gtyping.
-  - intros neA **; constructor; intros; split.
-
-
-
-
-
-
-
-
-
-
-
-
-
-
-
-
-(* Definition localConvL@{i j k l} Γ lA A (X Y : sigT@{Set l} (fun (C : term) => [LogRel@{i j k l} lA | Γ ||- A ≅ C])) : Type@{l} :=
-  [LogRel@{i j k l} lA | Γ ||- projT1@{Set l} X ≅ projT1@{Set l} Y]. *)
-
-(* Lemma convEquivLRPer@{i j k l i' j' k' l' v} Γ lA A A' (h : equivLR@{i j k l i' j' k' l' v} Γ lA A Γ lA A') : PER@{l l} (localConvL@{i j k l} Γ lA A).
-Proof.
-  constructor.
-  - intros [x ax] [y ay] xy. *)
 
 (** *** Equivalences of LRPack *)
 
@@ -1819,3 +1097,4 @@ Ltac irrelevance0 :=
 Ltac irrelevance := irrelevance0 ; [|eassumption] ; try first [reflexivity| now bsimpl].
 
 Ltac irrelevanceRefl := irrelevance0 ; [reflexivity|].
+*)
