theories/LogicalRelation/NormalRed.v
@@ -1,94 +1,102 @@
 From Coq Require Import CRelationClasses.
 From LogRel Require Import Utils Syntax.All GenericTyping LogicalRelation.
-From LogRel.LogicalRelation Require Import Induction Irrelevance Escape Reflexivity Weakening Neutral Transitivity Reduction EqRedRight.
+From LogRel.LogicalRelation Require Import Induction Irrelevance Escape Weakening Neutral Transitivity Reduction.
 
 Set Universe Polymorphism.
+Set Printing Primitive Projection Parameters.
 
-Ltac redSubst :=
-  match goal with
+Ltac redSubst t :=
+  repeat lazymatch goal with
   | [H : [_ |- ?X :⤳*: ?Y] |- _] =>
-    assert (X = Y)by (eapply redtywf_whnf ; gen_typing); subst; clear H
-  end.
-
+    try (unify t X;
+      assert (eeqsubst : X = Y) by (eapply redtywf_whnf ; gen_typing);
+      try (injection eeqsubst; intros); subst); block H
+  end; unblock.
 
 Section Normalization.
 Context `{GenericTypingProperties}.
 
-Set Printing Primitive Projection Parameters.
-
-Program Definition normRedNe0 {Γ A} (h : [Γ ||-ne A]) (wh : whne A) :
-  [Γ ||-ne A] :=
-  {| neRedTy.ty := A |}.
+Program Definition normRedNe0 {Γ A B} (h : [Γ ||-ne A ≅ B]) (wh : whne A) :
+  [Γ ||-ne A ≅ B] :=
+  {| neRedTy.tyL := A ; neRedTy.tyR := h.(neRedTy.tyR)|}.
 Next Obligation.
   pose proof (LRne_ zero h); escape; now eapply redtywf_refl.
 Qed.
-Next Obligation. destruct h; now redSubst. Qed.
+Next Obligation. now destruct h. Qed.
+Next Obligation. destruct h; cbn; now redSubst A. Qed.
 
 
-Program Definition normRedΠ0 {Γ F G l} (h : [Γ ||-Π<l> tProd F G])
-  : [Γ ||-Π<l> tProd F G] :=
-  {| PiRedTyPack.dom := F ;
-     PiRedTyPack.cod := G |}.
+Program Definition normRedΠl {Γ F G B l} (h : [Γ ||-Π<l> tProd F G ≅ B])
+  : [Γ ||-Π<l> tProd F G ≅ B] :=
+  {| ParamRedTy.domL := F ;
+     ParamRedTy.codL := G ;
+     ParamRedTy.domR := h.(ParamRedTy.domR) ;
+     ParamRedTy.codR := h.(ParamRedTy.codR) ; |}.
 Solve All Obligations with
-  intros; pose proof (e := redtywf_whnf (PiRedTyPack.red h) whnf_tProd);
-  symmetry in e; injection e; clear e;
-  destruct h ; intros; cbn in *; subst; eassumption.
+  (intros ; destruct h as [???? [] ?]; tea; cbn; redSubst (tProd F G); tea ;
+    constructor; tea; eapply redtywf_refl; gtyping).
 
-Program Definition normRedΣ0 {Γ F G l} (h : [Γ ||-Σ<l> tSig F G])
-  : [Γ ||-Σ<l> tSig F G] :=
-  {| PiRedTyPack.dom := F ;
-     PiRedTyPack.cod := G |}.
+Program Definition normRedΠr {Γ A F G l} (h : [Γ ||-Π<l> A ≅ tProd F G ])
+  : [Γ ||-Π<l> A ≅ tProd F G] :=
+  {| ParamRedTy.domR := F ;
+     ParamRedTy.codR := G ;
+     ParamRedTy.domL := h.(ParamRedTy.domL) ;
+     ParamRedTy.codL := h.(ParamRedTy.codL) ; |}.
 Solve All Obligations with
-  intros; pose proof (e := redtywf_whnf (PiRedTyPack.red h) whnf_tSig);
-  symmetry in e; injection e; clear e;
-  destruct h ; intros; cbn in *; subst; eassumption.
+  (intros ; destruct h as [???? ? []]; tea; cbn; redSubst (tProd F G); tea ;
+    constructor; tea; eapply redtywf_refl; gtyping).
 
-Definition normRedΠ {Γ F G l} (h : [Γ ||-<l> tProd F G]) : [Γ ||-<l> tProd F G] :=
-  LRPi' (normRedΠ0 (invLRΠ h)).
+Program Definition normRedΣl {Γ F G B l} (h : [Γ ||-Σ<l> tSig F G ≅ B])
+  : [Γ ||-Σ<l> tSig F G ≅ B] :=
+  {| ParamRedTy.domL := F ;
+     ParamRedTy.codL := G ;
+     ParamRedTy.domR := h.(ParamRedTy.domR) ;
+     ParamRedTy.codR := h.(ParamRedTy.codR) ; |}.
+Solve All Obligations with
+  (intros ; destruct h as [???? [] ?]; tea; cbn; redSubst (tSig F G); tea ;
+    constructor; tea; eapply redtywf_refl; gtyping).
+
+Program Definition normRedΣr {Γ F G B l} (h : [Γ ||-Σ<l> B ≅ tSig F G])
+  : [Γ ||-Σ<l> B ≅ tSig F G ] :=
+  {| ParamRedTy.domR := F ;
+     ParamRedTy.codR := G ;
+     ParamRedTy.domL := h.(ParamRedTy.domL) ;
+     ParamRedTy.codL := h.(ParamRedTy.codL) ; |}.
+Solve All Obligations with
+  (intros ; destruct h as [???? ? []]; tea; cbn; redSubst (tSig F G); tea ;
+    constructor; tea; eapply redtywf_refl; gtyping).
+
+
+Definition normRedΠ {Γ F F' G G' l} (h : [Γ ||-<l> tProd F G ≅ tProd F' G']) : [Γ ||-Π<l> tProd F G ≅ tProd F' G'] :=
+  normRedΠr (normRedΠl (invLRΠ h)).
+
+Definition normRedΣ {Γ F F' G G' l} (h : [Γ ||-<l> tSig F G ≅ tSig F' G']) : [Γ ||-Σ<l> tSig F G ≅ tSig F' G'] :=
+  normRedΣr (normRedΣl (invLRΣ h)).
+
 
 #[program]
-Definition normEqRedΠ {Γ F F' G G' l} (h : [Γ ||-<l> tProd F G])
-  (heq : [Γ ||-<l> _ ≅ tProd F' G' | h]) : [Γ ||-<l> _ ≅ tProd F' G' | normRedΠ h] :=
-  {|
-    PiRedTyEq.dom := F';
-    PiRedTyEq.cod := G';
-  |}.
+Definition normRedIdl {Γ A x y B l} (h : [Γ ||-Id<l> tId A x y ≅ B])
+  : [Γ ||-Id<l> tId A x y ≅ B] :=
+  {| IdRedTy.tyL := A ; IdRedTy.lhsL := x ; IdRedTy.rhsL := y ;
+     IdRedTy.tyR := h.(IdRedTy.tyR) ; IdRedTy.lhsR := h.(IdRedTy.lhsR) ; IdRedTy.rhsR := h.(IdRedTy.rhsR) ; |}.
 Solve All Obligations with
-  intros; assert[Γ ||-<l> _ ≅ tProd F' G' | normRedΠ h] as [?? red] by irrelevance;
-  pose proof (e := redtywf_whnf red whnf_tProd);
-  symmetry in e; injection e; clear e;
-  destruct h ; intros; cbn in *; subst; eassumption.
-
-Definition normRedΣ {Γ F G l} (h : [Γ ||-<l> tSig F G]) : [Γ ||-<l> tSig F G] :=
-  LRSig' (normRedΣ0 (invLRΣ h)).
+  intros ; destruct h ; tea; cbn; redSubst (tId A x y);
+  tea; first [now eapply irrLR | eapply redtywf_refl; gtyping].
 
 #[program]
-Definition normEqRedΣ {Γ F F' G G' l} (h : [Γ ||-<l> tSig F G])
-  (heq : [Γ ||-<l> _ ≅ tSig F' G' | h]) : [Γ ||-<l> _ ≅ tSig F' G' | normRedΣ h] :=
-  {|
-    PiRedTyEq.dom := F';
-    PiRedTyEq.cod := G';
-  |}.
+Definition normRedIdr {Γ A x y B l} (h : [Γ ||-Id<l> B ≅ tId A x y])
+  : [Γ ||-Id<l> B ≅ tId A x y] :=
+  {| IdRedTy.tyR := A ; IdRedTy.lhsR := x ; IdRedTy.rhsR := y ;
+     IdRedTy.tyL := h.(IdRedTy.tyL) ; IdRedTy.lhsL := h.(IdRedTy.lhsL) ; IdRedTy.rhsL := h.(IdRedTy.rhsL) ; |}.
 Solve All Obligations with
-  intros; assert[Γ ||-<l> _ ≅ tSig F' G' | normRedΣ h] as [?? red] by irrelevance;
-  pose proof (e := redtywf_whnf red whnf_tSig);
-  symmetry in e; injection e; clear e;
-  destruct h ; intros; cbn in *; subst; eassumption.
+  intros ; destruct h ; tea; cbn; redSubst (tId A x y);
+  tea; first [now eapply irrLR | eapply redtywf_refl; gtyping].
 
-#[program]
-Definition normRedId0 {Γ A x y l} (h : [Γ ||-Id<l> tId A x y])
-  : [Γ ||-Id<l> tId A x y] :=
-  mkIdRedTy A x y _ _ _ _.
-Solve All Obligations with
-  intros; pose proof (e := redtywf_whnf (IdRedTy.red h) whnf_tId);
-  symmetry in e; injection e; clear e;
-  destruct h ; intros; cbn in *; subst;
-  first [eassumption | irrelevance].
 
-Definition normRedId {Γ A x y l} (h : [Γ ||-<l> tId A x y]) : [Γ ||-<l> tId A x y] :=
-  LRId' (normRedId0 (invLRId h)).
+Definition normRedId {Γ A A' x x' y y' l} (h : [Γ ||-<l> tId A x y ≅ tId A' x' y']) : [Γ ||-Id<l> tId A x y ≅ tId A' x' y'] :=
+  normRedIdr (normRedIdl (invLRId h)).
 
-#[program]
+(* #[program]
 Definition normLambda {Γ F Fl Fr G tl tr l RΠ}
   (Rlam : [Γ ||-<l> tLambda Fl tl ≅ tLambda Fr tr : tProd F G | normRedΠ RΠ ]) :
   [Γ ||-<l> tLambda Fl tl ≅ tLambda Fr tr : tProd F G | normRedΠ RΠ ] :=
@@ -126,7 +134,7 @@ Definition invLRcan {Γ l A} (lr : [Γ ||-<l> A]) (w : isType A) : [Γ ||-<l> A]
   | SigType => fun _ x => LRSig' (normRedΣ0 x)
   | IdType => fun _ x => LRId' x
   | NeType wh => fun _ x => LRne_ _ (normRedNe0 x wh)
-  end lr (invLR lr (reflexivity A) w).
+  end lr (invLR lr (reflexivity A) w). *)
 
 End Normalization.
 
@@ -134,7 +142,7 @@ End Normalization.
 
 (* Normalizes a term reducible at a Π type *)
 
-Ltac normRedΠin X :=
+(* Ltac normRedΠin X :=
   let g := type of X in
   match g with
   (* | [ LRAd.pack ?R | _ ||- ?t : _] =>
@@ -193,4 +201,4 @@ Ltac normRedΣin X :=
     let X' := fresh X in
     rename X into X' ;
     assert (X : [_ ||-<_> t ≅ u : _ | LRSig' (normRedΣ0 (invLRΣ R))]) by irrelevance; clear X'
-  end.
+  end. *)
