theories/LogicalRelation/Introductions/Id.v
@@ -1,5 +1,5 @@
 From LogRel Require Import Utils Syntax.All GenericTyping LogicalRelation.
-From LogRel.LogicalRelation Require Import Induction Escape Irrelevance Weakening Neutral Reflexivity NormalRed Reduction Transitivity EqRedRight.
+From LogRel.LogicalRelation Require Import Properties.
 From LogRel.LogicalRelation.Introductions Require Import Universe.
 
 Set Universe Polymorphism.
@@ -8,23 +8,24 @@ Set Printing Primitive Projection Parameters.
 Section IdRed.
   Context `{GenericTypingProperties}.
 
-  Lemma IdRed0 {Γ l A t u} (RA : [Γ ||-<l> A]) :
-      [RA | Γ ||- t : _] ->
-      [RA | Γ ||- u : _] ->
-      [Γ ||-Id<l> tId A t u].
+  Lemma IdRed0 {Γ l A A' t t' u u'} (RA : [Γ ||-<l> A ≅ A']) :
+      [RA | Γ ||- t ≅ t' : _] ->
+      [RA | Γ ||- u ≅ u' : _] ->
+      [Γ ||-Id<l> tId A t u ≅ tId A' t' u'].
   Proof.
-    intros; eapply mkIdRedTy.
-    1: eapply redtywf_refl; escape; gen_typing.
-    all: tea.
+    intros; exists A A' t t' u u' RA; tea.
+    1,2: eapply redtywf_refl; escape; gtyping.
+    1: escape; gtyping.
+    typeclasses eauto.
   Defined.
 
-  Lemma IdRed {Γ l A t u} (RA : [Γ ||-<l> A]) :
-      [RA | Γ ||- t : _] ->
-      [RA | Γ ||- u : _] ->
-      [Γ ||-<l> tId A t u].
+  Lemma IdRed {Γ l A A' t t' u u'} (RA : [Γ ||-<l> A ≅ A']) :
+      [RA | Γ ||- t ≅ t' : _] ->
+      [RA | Γ ||- u ≅ u' : _] ->
+      [Γ ||-<l> tId A t u ≅ tId A' t' u'].
   Proof. intros; apply LRId'; now eapply IdRed0. Defined.
 
-  Lemma IdRedTy_inv {Γ l A t u} (RIA : [Γ ||-Id<l> tId A t u]) :
+  (* Lemma IdRedTy_inv {Γ l A t u B} (RIA : [Γ ||-Id<l> tId A t u]) :
     [× A = RIA.(IdRedTy.ty), t = RIA.(IdRedTy.lhs) & u = RIA.(IdRedTy.rhs)].
   Proof.
     pose proof (redtywf_whnf RIA.(IdRedTy.red) whnf_tId) as e; injection e; now split.
@@ -48,7 +49,7 @@ Section IdRed.
     + irrelevance.
     + cbn; rewrite <- elhs; irrelevance.
     + cbn; rewrite <- erhs; irrelevance.
-  Qed.
+  Qed. *)
 
   (* Lemma IdRedU@{i j k l} {Γ l A t u}
       (RU : [LogRel@{i j k l} l | Γ ||- U])
@@ -70,33 +71,24 @@ Section IdRed.
   Qed. *)
 
   Lemma IdCongRedU@{i j k l} {Γ l A A' t t' u u'}
-      (RU : [LogRel@{i j k l} l | Γ ||- U])
+      (RU : [LogRel@{i j k l} l | Γ ||- U ≅ U])
       (RU' := invLRU RU)
-      (RA : [LogRel@{i j k l} (URedTy.level RU') | Γ ||- A]) :
-    [RU | Γ ||- A : U] ->
+      (RA : [LogRel@{i j k l} (URedTy.level RU') | Γ ||- A ≅ A']) :
     [RU | _ ||- A ≅ A' : U] ->
     [RA | _ ||- t ≅ t' : _] ->
     [RA | _ ||- u ≅ u' : _] ->
     [RU | _ ||- tId A t u ≅ tId A' t' u' : U].
   Proof.
-    intros RAU RAAU' Rtt' Ruu'.
-    enough [LRU_ RU' | _ ||- tId A t u ≅ tId A' t' u': U] by irrelevance.
-    assert (hAA' : [RA | _ ||- A ≅ A']).
-    1: unshelve eapply UnivEqEq; try irrelevance + irrelevanceCum0.
-    escape. opector.
-    1,2: eexists (tId _ _ _); [eapply redtmwf_refl; gen_typing| constructor].
-    - eapply RedTyRecBwd; unshelve eapply IdRed.
-      all: try eapply lrefl; irrelevanceCum.
-    - pose proof (redtmwf_whnf (URedTm.red u0) whnf_tId) as <-.
-      pose proof (redtmwf_whnf (URedTm.red u1) whnf_tId) as <-.
-      now eapply convtm_Id.
-    - eapply RedTyRecBwd; unshelve eapply IdRed.
-      1: unshelve eapply UnivEq; [| |irrelevanceCum0| symmetry; irrelevanceCum].
-      all: eapply urefl; eapply LRTmEqConv; tea.
-    - eapply TyEqRecFwd.
-      unshelve eapply LRTyEqIrrelevantCum.
-      2: eapply RedTyRecFwd in l0 ; irrelevanceCum.
-      unshelve eapply IdCongRed; tea; gen_typing.
+    intros RAU Rtt' Ruu'.
+    enough [LRU_ RU' | _ ||- tId A t u ≅ tId A' t' u': U] by now eapply irrLREq.
+    escape.
+    unshelve eexists {| URedTm.te := tId A t u |} {| URedTm.te := tId A' t' u' |}; cbn.
+    2,4: constructor.
+    1,2: eapply redtmwf_refl.
+    1-3: gtyping.
+    unshelve eapply redTyRecBwd, IdRed.
+    1: now eapply cumLR.
+    all: now eapply irrLR.
   Qed.
 
 
@@ -125,30 +117,27 @@ Lemma reflRed' {Γ l A x} (RA : [Γ ||-<l> A]) (Rx : [RA | _ ||- x : _])
   (RIA := IdRed RA Rx Rx): [RIA | _ ||- tRefl A x : _].
 Proof. now eapply reflRed. Qed. *)
 
-Lemma reflCongRed {Γ l A A' x x'}
-  (RA : [Γ ||-<l> A])
-  (wtyA' : [ Γ |- A'])
-  (convAA' : [ Γ |- A ≅ A'])
-  (* (RAA : [RA | _ ||- _ ≅ A']) *)
+Lemma reflCongRed {Γ l A A0 A' B x x'}
+  (RA : [Γ ||-<l> A ≅ A0])
+  (wfA' : [Γ |- A'])
+  (eqA : [Γ |- A ≅ A'])
   (Rxx : [RA | _ ||- x ≅ x' : _])
-  (RIA : [Γ ||-<l> tId A x x]) :
+  (RIA : [Γ ||-<l> tId A x x ≅ B]) :
   [RIA | _ ||- tRefl A x ≅ tRefl A' x' : _].
 Proof.
-  set (RIA' := normRedId RIA).
-  enough [RIA' | _ ||- tRefl A x ≅ tRefl A' x' : _] by irrelevance.
+  set (RIA' := normRedIdl (invLRId RIA)).
+  enough [LRId' RIA' | _ ||- tRefl A x ≅ tRefl A' x' : _] by now eapply irrLREq.
   escape.
-  assert [Γ |- tId A' x' x' ≅ tId A x x] by (symmetry; timeout 1 gen_typing).
-  (* assert [Γ |- tId Ar xr xr ≅ tId A x x] by (symmetry; timeout 1 gen_typing). *)
+  assert [Γ |- tId A' x' x' ≅ tId A x x] by (symmetry; gtyping).
   exists (tRefl A x) (tRefl A' x').
-  1,2: eapply redtmwf_refl; unfold_id_outTy; cbn.
-  1: gen_typing.
-  1: eapply ty_conv; [|tea]; gen_typing.
-  1:  unfold_id_outTy; cbn; timeout 1 gen_typing.
+  1,2: eapply redtmwf_refl; cbn.
+  1: gtyping.
+  1: eapply ty_conv; [|tea]; gtyping.
+  1: cbn; gtyping.
   constructor; tea.
   1: eapply ty_conv; tea.
-  all: try irrelevance.
-  2,3: eapply lrefl; cbn; irrelevance.
-  now unshelve eapply escapeEq, reflLRTyEq.
+  1: cbn; now eapply lrefl.
+  all: first [now eapply irrLREq| now eapply lrefl, irrLREq].
 Qed.
 
 
@@ -158,52 +147,37 @@ Lemma reflCongRed' {Γ l A Al Ar x xl xr}
   (wtyAr : [Γ |- Ar])
   (convtyAAl : [Γ |- A ≅ Al])
   (convtyAAr : [Γ |- A ≅ Ar])
-  (* (RAAl : [RA | _ ||- _ ≅ Al])
-  (RAAr : [RA | _ ||- _ ≅ Ar]) *)
   (Rxxl : [RA | _ ||- x ≅ xl : _])
   (Rxxr : [RA | _ ||- x ≅ xr : _])
   (RIA : [Γ ||-<l> tId A x x]) :
   [RIA | _ ||- tRefl Al xl ≅ tRefl Ar xr : _].
-Proof. etransitivity; [symmetry|]; now eapply reflCongRed. Qed.
-
+Proof. etransitivity; [symmetry|]; now eapply (reflCongRed RA), irrLR. Qed.
 
 Lemma idElimPropCongRed {Γ l A A' x x' P P' hr hr' y y' e e'}
   (RA : [Γ ||-<l> A])
   (RA' : [Γ ||-<l> A'])
   (wtyA' := escape RA')
   (convtyAA' : [Γ |- A ≅ A' ])
-  (* (RAA' : [RA | Γ ||- A ≅ A']) *)
   (Rxx' : [RA | _ ||- x ≅ x' : _])
   (RIAxx : [Γ ||-<l> tId A x x])
   (RP0 : [Γ ,, A ,, tId A⟨@wk1 Γ A⟩ x⟨@wk1 Γ A⟩ (tRel 0) |- P])
   (RP0' : [Γ ,, A' ,, tId A'⟨@wk1 Γ A'⟩ x'⟨@wk1 Γ A'⟩ (tRel 0) |- P'])
   (RPP0 : [Γ ,, A ,, tId A⟨@wk1 Γ A⟩ x⟨@wk1 Γ A⟩ (tRel 0) |- P ≅ P'])
-  (RP : forall {y y' e e'} (Ryy' : [RA | Γ ||- y ≅ y' : _]) {RIAxy : [Γ ||-<l> tId A x y]},
-    [ RIAxy | _ ||- e ≅ e' : _] -> [Γ ||-<l> P[e .: y..]])
-  (RPP' : forall y y' e e'
+  (RP : forall {y y' e e'}
     (Ryy' : [RA | _ ||- y ≅ y' : _])
-    (RIAxy : [Γ ||-<l> tId A x y])
+    {RIAxy : [Γ ||-<l> tId A x y]}
     (Ree' : [ RIAxy | _ ||- e ≅ e' : _]),
-    [RP Ryy' Ree' | _ ||- P[e .: y..] ≅ P'[e' .: y'..]])
-  (RPeq : forall A' x' y y' e e'
-    (wtyA' : [Γ |- A' ])
-    (convtyAA' : [Γ |- A ≅ A' ])
-    (* (RAA' : [RA | _ ||- _ ≅ A']) *)
-    (Rxx' : [RA | _ ||- x ≅ x' : _])
-    (Ryy' : [RA | Γ ||- y ≅ y' : _])
-    (RIAxy : [Γ ||-<l> tId A x y])
-    (Ree' : [ RIAxy | _ ||- e ≅ e' : _]),
-    [RP Ryy' Ree' | Γ ||- P[e .: y..] ≅ P[e' .: y' ..]])
+    [Γ ||-<l> P[e .: y..] ≅ P'[e' .: y'..]])
   (Rrfl := (reflCongRed RA wtyA' convtyAA' Rxx' RIAxx))
   (Rhrhr' : [RP Rxx' Rrfl | _ ||- hr ≅ hr' : _])
   (Ryy' : [RA | _ ||- y ≅ y' : _])
   (RIAxy : [Γ ||-<l> tId A x y])
   (Ree' : [RIAxy | _ ||- e ≅ e' : _])
-  (Pee' : IdPropEq (normRedId0 (invLRId RIAxy)) e e') :
+  (Pee' : IdPropEq (normRedId RIAxy) e e') :
   [RP Ryy' Ree' | _ ||- tIdElim A x P hr y e ≅ tIdElim A' x' P' hr' y' e' : _].
 Proof.
-  pose proof (RPP' _ _ _ _ Rxx' _ Rrfl).
-  pose proof (RPP' _ _ _ _ Ryy' _ Ree').
+  pose proof (RP _ _ _ _ Rxx' _ Rrfl).
+  pose proof (RP _ _ _ _ Ryy' _ Ree').
   destruct Pee'; cbn in *; escape.
   - eapply redSubstTmEq; cycle 1.
     + eapply redtm_idElimRefl; tea.
@@ -211,31 +185,25 @@ Proof.
     + eapply redtm_idElimRefl; tea.
       1-4: eapply ty_conv; tea.
       1: transitivity A; tea; now symmetry.
-      2: eapply convtm_conv; tea; transitivity x; tea; now symmetry.
-      eapply convtm_conv; tea.
-      transitivity y; tea.
+      2: eapply convtm_conv; [transitivity x; tea; now symmetry|tea].
+      eapply convtm_conv; [transitivity y; tea|tea].
       transitivity x0; symmetry; tea.
-      transitivity x; tea. now symmetry.
-    + unshelve eapply escapeEq, RPP'; tea.
-    + eapply LRTmEqConv; tea.
-      irrelevanceRefl.
-      eapply RPeq; cycle 1; tea.
-      Unshelve.
-      * transitivity x0; [|symmetry]; irrelevance.
-      * tea.
-      * now eapply reflCongRed.
-  - eapply neuTermEq.
+      transitivity x; tea; now symmetry.
+    + eapply irrLRConv; tea.
+      etransitivity; [|symmetry]; eapply RP.
+      4: now eapply lrefl.
+      1,3: eapply irrLR; first [eapply e| eapply e1].
+      eapply reflCongRed; tea.
+      Unshelve. tea.
+  - eapply reflectLR.
     + now eapply ty_IdElim.
     + eapply ty_conv; [|symmetry; tea].
       eapply ty_IdElim; tea.
       all: eapply ty_conv; tea.
       now eapply convty_Id.
     + eapply convneu_IdElim; tea.
-      destruct r; unfold_id_outTy; now cbn in *.
+      destruct r;  now cbn in *.
 Qed.
-
-
-
 
 
 Lemma idElimCongRed {Γ l A A' x x' P P' hr hr' y y' e e'}
@@ -243,28 +211,16 @@ Lemma idElimCongRed {Γ l A A' x x' P P' hr hr' y y' e e'}
   (RA' : [Γ ||-<l> A'])
   (wtyA' := escape RA')
   (convtyAA' : [Γ |- A ≅ A' ])
-  (* (RAA' : [RA | Γ ||- A ≅ A']) *)
   (Rxx' : [RA | _ ||- x ≅ x' : _])
   (RIAxx : [Γ ||-<l> tId A x x])
   (RP0 : [Γ ,, A ,, tId A⟨@wk1 Γ A⟩ x⟨@wk1 Γ A⟩ (tRel 0) |- P])
   (RP0' : [Γ ,, A' ,, tId A'⟨@wk1 Γ A'⟩ x'⟨@wk1 Γ A'⟩ (tRel 0) |- P'])
   (RPP0 : [Γ ,, A ,, tId A⟨@wk1 Γ A⟩ x⟨@wk1 Γ A⟩ (tRel 0) |- P ≅ P'])
-  (RP : forall {y y' e e'} (Ryy' : [RA | Γ ||- y ≅ y' : _]) {RIAxy : [Γ ||-<l> tId A x y]},
-    [ RIAxy | _ ||- e ≅ e' : _] -> [Γ ||-<l> P[e .: y..]])
-  (RPP' : forall y y' e e'
+  (RP : forall {y y' e e'}
     (Ryy' : [RA | _ ||- y ≅ y' : _])
-    (RIAxy : [Γ ||-<l> tId A x y])
+    {RIAxy : [Γ ||-<l> tId A x y]}
     (Ree' : [ RIAxy | _ ||- e ≅ e' : _]),
-    [RP Ryy' Ree' | _ ||- P[e .: y..] ≅ P'[e' .: y'..]])
-  (RPeq : forall A' x' y y' e e'
-    (wtyA' : [Γ |- A' ])
-    (convtyAA' : [Γ |- A ≅ A' ])
-    (* (RAA' : [RA | _ ||- _ ≅ A']) *)
-    (Rxx' : [RA | _ ||- x ≅ x' : _])
-    (Ryy' : [RA | Γ ||- y ≅ y' : _])
-    (RIAxy : [Γ ||-<l> tId A x y])
-    (Ree' : [ RIAxy | _ ||- e ≅ e' : _]),
-    [RP Ryy' Ree' | Γ ||- P[e .: y..] ≅ P[e' .: y' ..]])
+    [Γ ||-<l> P[e .: y..] ≅ P'[e' .: y'..]])
   (Rrfl := (reflCongRed RA wtyA' convtyAA' Rxx' RIAxx))
   (Rhrhr' : [RP Rxx' Rrfl | _ ||- hr ≅ hr' : _])
   (Ryy' : [RA | _ ||- y ≅ y' : _])
@@ -272,27 +228,22 @@ Lemma idElimCongRed {Γ l A A' x x' P P' hr hr' y y' e e'}
   (Ree' : [RIAxy | _ ||- e ≅ e' : _]) :
   [RP Ryy' Ree' | _ ||- tIdElim A x P hr y e ≅ tIdElim A' x' P' hr' y' e' : _].
 Proof.
-  assert (nRee' : [normRedId RIAxy | Γ ||- e ≅ e' : _]) by irrelevance.
-  destruct nRee' as [nfL nfR ??? prop]; unfold_id_outTy; cbn in *.
-  pose proof (RPP' _ _ _ _ Rxx' _ Rrfl).
-  pose proof (RPP' _ _ _ _ Ryy' _ Ree').
-  pose proof (IdPropEq_whnf _ _ _ prop) as [].
-  assert (RenfL : [RIAxy | _ ||- e ≅ nfL : _]).
-  1: symmetry; eapply redTmEqFwd; tea; now eapply lrefl.
-  assert (RnfLR : [RIAxy | _ ||- nfL ≅ nfR : _])
-  by (eapply redTmEqFwdBoth; cycle 1; tea).
-  assert (Ryy : [RA | _ ||- y ≅ y : _]) by now eapply lrefl.
-  pose proof (RAA := reflLRTyEq RA).
-  pose proof (RPeq _ _ _ _ _ _ wtyA' convtyAA' Rxx' Ryy _ RenfL).
-  escape.
-  assert [Γ |- tId A x y ≅ tId A' x' y'] by gen_typing.
-  eapply redSubstTmEq; cycle 1; tea.
-  1,2: eapply redtm_idElim; tea.
-  1: gen_typing.
-  1-3: now eapply ty_conv.
-  1: eapply redtm_conv; tea; gen_typing.
-  eapply LRTmEqConv. 1: now eapply LRTyEqSym.
-  now unshelve eapply idElimPropCongRed.
+  assert (nRee' : [LRId' (normRedId RIAxy) | Γ ||- e ≅ e' : _]) by now eapply irrLREq.
+  pose proof (redTmFwd' nRee') as [].
+  eapply redSubstTmEq.
+  + eapply irrLRConv.
+    2: unshelve (eapply idElimPropCongRed; cycle 3; tea; exact (nRee'.(IdRedTmEq.prop)));
+     [|tea|now eapply irrLR].
+    etransitivity; [|symmetry]; eapply RP; cycle 1; [now eapply lrefl| tea..].
+  + escape; eapply redtm_idElim; tea; eapply tmr_wf_red; exact (whredtmL nRee').(tmred_whnf_red).
+  + escape; eapply redtm_idElim; tea.
+    1,3: now eapply ty_conv.
+    2: eapply redtm_conv; [eapply tmr_wf_red; exact (whredtmR nRee').(tmred_whnf_red)|].
+    2: unfold IdRedTy.outTy; cbn; gtyping.
+    eapply ty_conv; tea; eapply escapeEq, RP; tea.
 Qed.
+
+
+
 
 End IdRed.
