theories/LogicalRelation/Introductions/SimpleArr.v
@@ -1,6 +1,6 @@
 From LogRel Require Import Utils Syntax.All GenericTyping LogicalRelation.
-From LogRel.LogicalRelation Require Import Induction Irrelevance Weakening Neutral Escape Reflexivity NormalRed Reduction Transitivity Application.
-From LogRel.LogicalRelation.Introductions Require Import Poly Pi.
+From LogRel.LogicalRelation Require Import Properties.
+From LogRel.LogicalRelation.Introductions Require Import Poly Pi Application.
 
 Set Universe Polymorphism.
 Set Printing Primitive Projection Parameters.
@@ -8,111 +8,28 @@ Set Printing Primitive Projection Parameters.
 Section SimpleArrow.
   Context `{GenericTypingProperties}.
 
-  Lemma shiftPolyRed {Γ l A B} : [Γ ||-<l> A] -> [Γ ||-<l> B] -> PolyRed Γ l A B⟨↑⟩.
+  Lemma shiftPolyRed {Γ l A A' B B'} : [Γ ||-<l> A ≅ A'] -> [Γ ||-<l> B ≅ B'] -> PolyRed Γ l A A' B⟨↑⟩ B'⟨↑⟩.
   Proof.
     intros; escape; unshelve econstructor.
-    - intros; now eapply wk.
-    - intros; bsimpl; rewrite <- rinstInst'_term; now eapply wk.
-    - now escape.
-    - renToWk; eapply wft_wk; gen_typing.
-    - intros; irrelevance0.
-      2: replace (subst_term _ _) with B⟨ρ⟩.
-      2: eapply wkEq, reflLRTyEq.
-      all: bsimpl; now rewrite rinstInst'_term.
-      Unshelve. all: tea.
+    - intros; now eapply wkLR.
+    - intros; rewrite 2!shift_subst_scons; now eapply wkLR.
   Qed.
 
-
-  Lemma ArrRedTy0 {Γ l A B} : [Γ ||-<l> A] -> [Γ ||-<l> B] -> [Γ ||-Π<l> arr A B].
+  Lemma ArrRedTy0 {Γ l A A' B B'} : [Γ ||-<l> A ≅ A'] -> [Γ ||-<l> B ≅ B'] -> [Γ ||-Π<l> arr A B ≅ arr A' B'].
   Proof.
     intros RA RB.
-    now apply LRPiPoly0, shiftPolyRed.
+    eapply LRPiPoly0, shiftPolyRed; tea; escape; gtyping.
   Qed.
 
-  Lemma ArrRedTy {Γ l A B} : [Γ ||-<l> A] -> [Γ ||-<l> B] -> [Γ ||-<l> arr A B].
+  Lemma ArrRedTy {Γ l A A' B B'} : [Γ ||-<l> A ≅ A'] -> [Γ ||-<l> B ≅ B'] -> [Γ ||-<l> arr A B ≅ arr A' B'].
   Proof. intros; eapply LRPi'; now eapply ArrRedTy0. Qed.
 
-  Lemma shiftPolyRedEq {Γ l A A' B B'} (RA : [Γ ||-<l> A]) (RB : [Γ ||-<l> B]) (PAB : PolyRed Γ l A B⟨↑⟩) :
-    [Γ ||-<l> A ≅ A' | RA] ->
-    [Γ ||-<l> B ≅ B' | RB] ->
-    PolyRedEq PAB A' B'⟨↑⟩.
+  Lemma polyRedArrExt {Γ l A A' B B' C C'} : PolyRed Γ l A A' B B' -> PolyRed Γ l A A' C C' -> PolyRed Γ l A A' (arr B C) (arr B' C').
   Proof.
-    intros; escape; unshelve econstructor.
-    - intros; irrelevanceRefl; now eapply wkEq.
-    - intros; irrelevance0; rewrite shift_subst_scons; [reflexivity|].
-      now eapply wkEq.
-      Unshelve. all: tea.
+    intros [RA RB] [RA' RC]; unshelve econstructor; tea.
+    now unshelve (intros; rewrite 2!subst_arr; eapply ArrRedTy; [eapply RB|eapply RC]; tea; now eapply irrLR).
   Qed.
 
-  Lemma arrRedCong0 {Γ l A A' B B'} (RA : [Γ ||-<l> A]) (RB : [Γ ||-<l> B])
-    (tyA' : [Γ |- A']) (tyB' : [Γ |- B']) (RAB : [Γ ||-Π<l> arr A B]) :
-    [Γ ||-<l> A ≅ A' | RA] ->
-    [Γ ||-<l> B ≅ B' | RB] ->
-    [Γ ||-Π arr A B ≅ arr A' B' | normRedΠ0 RAB].
-  Proof.
-    intros RAA' RBB'; escape.
-    unshelve econstructor; cycle 2.
-    + eapply redtywf_refl; now eapply wft_simple_arr.
-    + now cbn.
-    + now eapply convty_simple_arr.
-    + now eapply shiftPolyRedEq.
-  Qed.
-
-
-  Lemma arrRedCong {Γ l A A' B B'} (RA : [Γ ||-<l> A]) (RB : [Γ ||-<l> B])
-    (tyA' : [Γ |- A']) (tyB' : [Γ |- B']) :
-    [Γ ||-<l> A ≅ A' | RA] ->
-    [Γ ||-<l> B ≅ B' | RB] ->
-    [Γ ||-<l> arr A B ≅ arr A' B' | normRedΠ (ArrRedTy RA RB)].
-  Proof.
-    intros; now eapply arrRedCong0.
-  Qed.
-
-  Lemma arrRedCong' {Γ l A A' B B'} (RA : [Γ ||-<l> A]) (RB : [Γ ||-<l> B])
-    (tyA' : [Γ |- A']) (tyB' : [Γ |- B']) (RAB : [Γ ||-<l> arr A B]) :
-    [Γ ||-<l> A ≅ A' | RA] ->
-    [Γ ||-<l> B ≅ B' | RB] ->
-    [Γ ||-<l> arr A B ≅ arr A' B' | RAB].
-  Proof.
-    intros; irrelevanceRefl; now eapply arrRedCong.
-  Qed.
-
-
-  Lemma polyRedArrExt {Γ l A B C} : PolyRed Γ l A B -> PolyRed Γ l A C -> PolyRed Γ l A (arr B C).
-  Proof.
-    intros [tyA tyB RA RB RBext] [_ tyC RA' RC RCext].
-    opector; tea.
-    2: now eapply wft_simple_arr.
-    + intros; rewrite subst_arr; refold.
-      apply ArrRedTy; [eapply RB| eapply RC]; now irrelevanceRefl.
-      Unshelve. all: tea.
-    + intros.
-      irrelevance0; rewrite subst_arr; [refold; reflexivity|]; refold.
-      eapply arrRedCong.
-      1,2: eapply escape; first [eapply RB| eapply RC]; symmetry; now irrelevanceRefl.
-      1,2: first [eapply RBext| eapply RCext]; now irrelevanceRefl.
-      Unshelve. all: now irrelevanceRefl + tea.
-  Qed.
-
-  Lemma polyRedEqArrExt {Γ l A A' B B' C C'}
-    (PAB : PolyRed Γ l A B) (PAC : PolyRed Γ l A C)
-    (PAB' : PolyRed Γ l A' B') (PAC' : PolyRed Γ l A' C')
-    (PABC : PolyRed Γ l A (arr B C))
-    (PABeq : PolyRedEq PAB A' B')
-    (PACeq : PolyRedEq PAC A' C')
-    : PolyRedEq PABC A' (arr B' C').
-  Proof.
-    constructor.
-    + intros; irrelevanceRefl; now unshelve eapply (PolyRedEq.shpRed PABeq).
-    + intros; irrelevance0; rewrite subst_arr; refold; [reflexivity|].
-      apply arrRedCong.
-      * eapply escape; unshelve eapply (PolyRed.posRed); cycle 1; tea.
-        eapply LRTmEqConv ; tea; irrelevanceRefl; now unshelve eapply (PolyRedEq.shpRed PABeq).
-      * eapply escape; unshelve eapply (PolyRed.posRed); cycle 1; tea.
-        eapply LRTmEqConv; tea; irrelevanceRefl; now unshelve eapply (PolyRedEq.shpRed PABeq).
-      * unshelve eapply (PolyRedEq.posRed PABeq); tea; now irrelevanceRefl.
-      * unshelve eapply (PolyRedEq.posRed PACeq); tea; now irrelevanceRefl.
-  Qed.
 
 
   (* Section SimpleAppTerm.
@@ -159,18 +76,16 @@ Section SimpleArrow.
   Qed. *)
 
 
-  Lemma simple_appcongTerm {Γ t t' u u' F G l}
-    {RF : [Γ ||-<l> F]}
-    (RG : [Γ ||-<l> G])
-    (RΠ : [Γ ||-<l> arr F G])
+  Lemma simple_appcongTerm {Γ t t' u u' F F' G G' l}
+    {RF : [Γ ||-<l> F ≅ F']}
+    (RG : [Γ ||-<l> G ≅ G'])
+    (RΠ : [Γ ||-<l> arr F G ≅ arr F' G'])
     (Rtt' : [Γ ||-<l> t ≅ t' : _ | RΠ])
     (Ruu' : [Γ ||-<l> u ≅ u' : F | RF ]) :
       [Γ ||-<l> tApp t u ≅ tApp t' u' : G | RG].
   Proof.
-    irrelevance0.
-    2: eapply appcongTerm; tea.
-    now bsimpl.
-    Unshelve. now bsimpl.
+    unshelve (eapply irrLREq, appcongTerm; tea);
+    erewrite !shift_subst1; [now eapply lrefl|reflexivity].
   Qed.
 
   (* Lemma wkRedArr {Γ l A B f}
