theories/LogicalRelation/Properties.v
@@ -1,0 +1,4 @@
+From Coq Require Export CRelationClasses.
+From LogRel Require Export LogicalRelation.
+From LogRel.LogicalRelation Require Export Induction Escape Irrelevance Symmetry Transitivity Weakening Neutral Reduction InstKripke NormalRed.
+
